theories/embedding/types.v
@@ -2,15 +2,69 @@ From fae_gtlc_mu Require Import stlc_mu.typing.
 From fae_gtlc_mu Require Import cast_calculus.types.
 
 Reserved Notation "[| τ |]" (at level 4, τ at next level).
-Fixpoint embed_type (τ : stlc_mu.typing.type) : type :=
+Fixpoint embed_type (τ : stlc_mu.types.type) : type :=
   match τ with
-  | typing.TUnit => TUnit
-  | typing.TProd τ1 τ2 => TProd [| τ1 |] [| τ2 |]
-  | typing.TSum τ1 τ2 => TSum [| τ1 |] [| τ2 |]
-  | typing.TArrow τ1 τ2 => TArrow [| τ1 |] [| τ2 |]
-  | typing.TRec τb => TRec [| τb |]
-  | typing.TVar x => TVar x
+  | stlc_mu.types.TUnit => TUnit
+  | stlc_mu.types.TProd τ1 τ2 => TProd [| τ1 |] [| τ2 |]
+  | stlc_mu.types.TSum τ1 τ2 => TSum [| τ1 |] [| τ2 |]
+  | stlc_mu.types.TArrow τ1 τ2 => TArrow [| τ1 |] [| τ2 |]
+  | stlc_mu.types.TRec τb => TRec [| τb |]
+  | stlc_mu.types.TVar x => TVar x
   end where "[| e |]" := (embed_type e).
 
-Lemma embed_through_unfold τ : [| τ.[typing.TRec τ/] |] = [| τ |].[TRec [| τ |]/].
-Admitted.
+Lemma etype_ren_gen τ :
+  forall k l, [| τ.[upn l (ren (+k))] |] = [|τ|].[upn l (ren (+k))].
+Proof.
+  induction τ; intros k l; try by asimpl.
+  - asimpl. by rewrite IHτ1 IHτ2.
+  - asimpl. by rewrite IHτ1 IHτ2.
+  - asimpl. by rewrite IHτ1 IHτ2.
+  - simpl. specialize (IHτ k (S l)). by rewrite IHτ.
+  - asimpl. do 2 rewrite (iter_up l x (ren (+k))).
+    destruct (lt_dec x l); by asimpl.
+Qed.
+
+Lemma embd_unfold_comm_gen (τb : stlc_mu.types.type) : forall (τ : stlc_mu.types.type) k,
+  [| τb.[upn k (τ .: ids)] |] = [|τb|].[upn k ([|τ|] .: ids)].
+Proof.
+  induction τb; intros τ' k; try by asimpl.
+  - asimpl. by rewrite IHτb1 IHτb2.
+  - asimpl. by rewrite IHτb1 IHτb2.
+  - asimpl. by rewrite IHτb1 IHτb2.
+  - simpl. specialize (IHτb τ' (S k)). by rewrite IHτb.
+  - asimpl.
+    rewrite (iter_up k x (τ' .: ids)) (iter_up k x ([|τ'|] .: ids)).
+    destruct (lt_dec x k).
+      + by asimpl.
+      + destruct (decide (x - k = 0)); asimpl. rewrite e. asimpl.
+        cut ([| τ'.[upn 0 (ren (+k))] |] = ([| τ' |]).[upn 0 (ren (+k))]).
+        by asimpl. by rewrite etype_ren_gen.
+        destruct (x - k). exfalso; lia. by asimpl.
+Qed.
+
+Lemma embd_unfold_comm (τb : stlc_mu.types.type) :
+  [| τb.[stlc_mu.types.TRec τb/]|] = [|τb|].[TRec [|τb|]/].
+Proof.
+  cut ([| (τb.[upn 0 ((stlc_mu.types.TRec τb) .: ids)])|] = [|τb|].[upn 0 ([|(stlc_mu.types.TRec τb)|] .: ids)]).
+  by asimpl. apply embd_unfold_comm_gen.
+Qed.
+
+Lemma embd_closed_gen τ : forall n (pnτ : stlc_mu.types.TnClosed n τ), TnClosed n [|τ|].
+Proof.
+  induction τ; intros n pnτ; simpl; try by (intro σ; by asimpl).
+  - specialize (IHτ1 n (stlc_mu.types.TProd_nclosed1 pnτ)).
+    specialize (IHτ2 n (stlc_mu.types.TProd_nclosed2 pnτ)).
+    intro σ; asimpl; by rewrite IHτ1 IHτ2.
+  - specialize (IHτ1 n (stlc_mu.types.TSum_nclosed1 pnτ)).
+    specialize (IHτ2 n (stlc_mu.types.TSum_nclosed2 pnτ)).
+    intro σ; asimpl; by rewrite IHτ1 IHτ2.
+  - specialize (IHτ1 n (stlc_mu.types.TArrow_nclosed1 pnτ)).
+    specialize (IHτ2 n (stlc_mu.types.TArrow_nclosed2 pnτ)).
+    intro σ; asimpl; by rewrite IHτ1 IHτ2.
+  - specialize (IHτ (S n) (stlc_mu.types.TRec_nclosed1 pnτ)).
+    intro σ; asimpl; by rewrite IHτ.
+  - apply TnClosed_var. by apply stlc_mu.types.TnClosed_var.
+Qed.
+
+Lemma embd_closed {τ} (pτ : stlc_mu.types.TClosed τ) : TClosed [|τ|].
+Proof. apply (embd_closed_gen τ 0 pτ). Qed.
