theories/fae.v
@@ -1,8 +1,8 @@
-From fae_gtlc_mu.stlc_mu Require Export contexts.
-From fae_gtlc_mu.cast_calculus Require Export contexts.
-From fae_gtlc_mu.embedding Require Export expressions types.
-From fae_gtlc_mu.backtranslation Require Export contexts.
-From fae_gtlc_mu.refinements.static_gradual Require Export soundness.
+From fae_gtlc_mu.stlc_mu Require Export contexts typing.
+From fae_gtlc_mu.cast_calculus Require Export contexts typing.
+From fae_gtlc_mu.embedding Require Export expressions types well_typedness.
+From fae_gtlc_mu.backtranslation Require Export contexts well_typedness.
+From fae_gtlc_mu.refinements.static_gradual Require Export adequacy.
 From fae_gtlc_mu.refinements.static_gradual Require Export rel_ref_specs.
 
 Notation "Γ ⊨ e '=ctx-grad=' e' : τ" :=
@@ -11,40 +11,52 @@ Notation "Γ ⊨ e '=ctx-grad=' e' : τ" :=
 Notation "Γ ⊨ e '=ctx-stat=' e' : τ" :=
   (stlc_mu.contexts.ctx_equiv Γ e e' τ) (at level 74, e, e', τ at next level).
 
-Lemma static_ctx_refines_gradual (Γ : list stlc_mu.typing.type) (e : stlc_mu.lang.expr) (τ : stlc_mu.typing.type) (de : Γ ⊢ₛ e : τ) :
+Lemma static_ctx_refines_gradual (Γ : list stlc_mu.types.type) (e : stlc_mu.lang.expr) (τ : stlc_mu.types.type) (de : Γ ⊢ₛ e : τ) :
   ∀ (Cₜ : cast_calculus.contexts.ctx), cast_calculus.contexts.typed_ctx Cₜ (map embed_type Γ) (embed_type τ) [] TUnit →
      Halts_stat (stlc_mu.contexts.fill_ctx (backtranslate_ctx Cₜ) e) →
      Halts_grad (fill_ctx Cₜ [[e]]).
 Proof.
   intros Cₜ dCₜ Hs.
-  apply (@soundness actualΣ _ _ (stlc_mu.contexts.fill_ctx (backtranslate_ctx Cₜ) e) _ TUnit).
-  intros.
-  eapply back_ctx_relates. admit. admit. apply dCₜ.
-  apply embedding_relates; done.
-  done.
-Admitted.
+  apply (@adequacy actualΣ _ _ (stlc_mu.contexts.fill_ctx (backtranslate_ctx Cₜ) e) _ TUnit); auto. intros.
+  apply (back_ctx_relates (map embed_type Γ) _ _ (embed_type τ)); auto. apply (embd_closed (stlc_mu.typing.typed_closed de)).
+  by apply embedding_relates.
+Qed.
 
-Lemma gradual_ctx_refines_static (Γ : list stlc_mu.typing.type) (e : stlc_mu.lang.expr) (τ : stlc_mu.typing.type) :
+Lemma gradual_ctx_refines_static (Γ : list stlc_mu.types.type) (e : stlc_mu.lang.expr) (τ : stlc_mu.types.type) :
   ∀ (K : cast_calculus.contexts.ctx), cast_calculus.contexts.typed_ctx K (map embed_type Γ) (embed_type τ) [] TUnit →
      Halts_grad (fill_ctx K [[e]]) →
      Halts_stat (stlc_mu.contexts.fill_ctx (backtranslate_ctx K) e).
 Proof.
 Admitted.
 
+Definition retract τ : backtranslate_type (embed_type τ) = τ.
+Proof. induction τ; simpl; try done; try by rewrite IHτ1 IHτ2. by rewrite IHτ. Qed.
 
 Theorem ctx_eq_preservation Γ e1 e2 τ (Hctx : Γ ⊨ e1 =ctx-stat= e2 : τ) :
   map embed_type Γ ⊨ [[e1]] =ctx-grad= [[e2]] : embed_type τ.
 Proof.
-  split; try split. admit. admit.
+  assert (pe1 : Γ ⊢ₛ e1 : τ). apply Hctx. assert (pe2 : Γ ⊢ₛ e2 : τ). apply Hctx.
+  split; try split; try by apply embedding.well_typedness.well_typedness_expr.
   intros Cₜ dCₜ. split.
   - intro Hg1.
     apply (static_ctx_refines_gradual Γ e2 τ (ltac:(apply Hctx)) Cₜ dCₜ).
-    apply Hctx. admit.
-    apply (gradual_ctx_refines_static Γ e1 τ Cₜ dCₜ).
-    apply Hg1.
+    apply Hctx.
+    cut (stlc_mu.contexts.typed_ctx
+           (backtranslate_ctx Cₜ)
+           (map backtranslate_type (map embed_type Γ)) (backtranslate_type $ embed_type τ)
+           (map backtranslate_type []) (backtranslate_type $ embed_type stlc_mu.types.TUnit)).
+    repeat rewrite retract. rewrite map_map (map_ext _ id _ (Γ)). by rewrite (map_id Γ). intro; by rewrite retract.
+    apply well_typedness_ctx. apply (embd_closed (stlc_mu.typing.typed_closed pe1)). auto.
+    by apply (gradual_ctx_refines_static Γ e1 τ Cₜ dCₜ).
   - intro Hg2.
     apply (static_ctx_refines_gradual Γ e1 τ (ltac:(apply Hctx)) Cₜ dCₜ).
-    apply Hctx. admit.
+    apply Hctx.
+    cut (stlc_mu.contexts.typed_ctx
+           (backtranslate_ctx Cₜ)
+           (map backtranslate_type (map embed_type Γ)) (backtranslate_type $ embed_type τ)
+           (map backtranslate_type []) (backtranslate_type $ embed_type stlc_mu.types.TUnit)).
+    repeat rewrite retract. rewrite map_map (map_ext _ id _ (Γ)). by rewrite (map_id Γ). intro; by rewrite retract.
+    apply well_typedness_ctx. apply (embd_closed (stlc_mu.typing.typed_closed pe1)). auto.
     apply (gradual_ctx_refines_static Γ e2 τ Cₜ dCₜ).
     apply Hg2.
-Admitted.
+Qed.
