theories/stlc_mu/typing.v
@@ -3,112 +3,72 @@ From fae_gtlc_mu Require Export prelude.
 From fae_gtlc_mu.stlc_mu Require Export types lang.
 From Coq Require Import List.
 
-(* other options {{{
+(* We make typing derivations such that given Γ ⊢ₛ e : τ, τ is closed.
+   a Γ can -- in principle -- contain open types, but such open types will never be used in the typing derivation.
+   So, morally, we can think of Γ as satisfying Forall TClosed *)
 
-  Disadvantage here; in general we do not have [τ&pτ] = [τ&pτ'] without assuming proof irrelevance..
+Reserved Notation "Γ ⊢ₛ e : τ" (at level 74, e, τ at next level).
 
-  Definition ctype := Ssig (fun τ => Squash (TClosed τ)).
+Inductive typed (Γ : list type) : expr → type → Prop :=
+  | Var_typed x τ (pτ : TClosed τ) : (Γ !! x = Some τ) → Γ ⊢ₛ Var x : τ
+  | Unit_typed : Γ ⊢ₛ Unit : TUnit
+  | Pair_typed e1 e2 τ1 τ2 :
+     Γ ⊢ₛ e1 : τ1 → Γ ⊢ₛ e2 : τ2 → Γ ⊢ₛ Pair e1 e2 : TProd τ1 τ2
+  | Fst_typed e τ1 τ2 : Γ ⊢ₛ e : TProd τ1 τ2 → Γ ⊢ₛ Fst e : τ1
+  | Snd_typed e τ1 τ2 : Γ ⊢ₛ e : TProd τ1 τ2 → Γ ⊢ₛ Snd e : τ2
+  | InjL_typed e τ1 τ2 (pτ2 : TClosed τ2) : Γ ⊢ₛ e : τ1 → Γ ⊢ₛ InjL e : TSum τ1 τ2
+  | InjR_typed e τ1 (pτ1 : TClosed τ1) τ2 : Γ ⊢ₛ e : τ2 → Γ ⊢ₛ InjR e : TSum τ1 τ2
+  | Case_typed e0 e1 e2 τ1 τ2 ρ :
+     Γ ⊢ₛ e0 : TSum τ1 τ2 → τ1 :: Γ ⊢ₛ e1 : ρ → τ2 :: Γ ⊢ₛ e2 : ρ →
+     Γ ⊢ₛ Case e0 e1 e2 : ρ
+  | Lam_typed e τ1 (pτ1 : TClosed τ1) τ2 : τ1 :: Γ ⊢ₛ e : τ2 → Γ ⊢ₛ Lam e : TArrow τ1 τ2
+  | App_typed e1 e2 τ1 τ2 : Γ ⊢ₛ e1 : TArrow τ1 τ2 → Γ ⊢ₛ e2 : τ1 → Γ ⊢ₛ App e1 e2 : τ2
+  | Fold_typed e τ : Γ ⊢ₛ e : τ.[TRec τ/] → Γ ⊢ₛ Fold e : TRec τ
+  | Unfold_typed e τ : Γ ⊢ₛ e : TRec τ → Γ ⊢ₛ Unfold e : τ.[TRec τ/]
+where "Γ ⊢ₛ e : τ" := (typed Γ e τ).
 
-  Only allows you to access the closed field in SProp...
-  So typed must live in SProp as well.
-  When doing induction on typed, we must be in SProp as well... etc.
+Lemma typed_closed {Γ} {e} {τ} : Γ ⊢ₛ e : τ → TClosed τ.
+Proof.
+  intro d. induction d.
+  - auto.
+  - apply TUnit_TClosed.
+  - by apply TProd_closed.
+  - by eapply TProd_closed1.
+  - by eapply TProd_closed2.
+  - by eapply TSum_closed.
+  - by eapply TSum_closed.
+  - auto.
+  - by apply TArrow_closed.
+  - by eapply TArrow_closed2.
+  - by apply closed_Fold_typed_help.
+  - by apply TRec_closed_unfold.
+Qed.
 
-  Add clause to allow for if Squash τ = τ', then we can interchange...
+Lemma Unfold_Fold_typed Γ e τ :
+  Γ ⊢ₛ e : τ → Γ ⊢ₛ Unfold (Fold e) : τ.
+Proof.
+  intro.
+  rewrite -(typed_closed H (TRec τ .: ids)).
+  apply Unfold_typed.
+  apply Fold_typed.
+  by rewrite (typed_closed H (TRec τ .: ids)).
+Qed.
 
-  Advantage here; works well for type checking; proofs will get shelved..
-}}} *)
+Lemma Unfold_typed_eq Γ e τb τ' : (τb.[TRec τb/] = τ') →
+  Γ ⊢ₛ e : (TRec τb) →
+  Γ ⊢ₛ Unfold e : τ'.
+Proof. intros eq d. rewrite -eq. by apply Unfold_typed. Qed.
+
+Lemma rewrite_typed {Γ e τ τ'} :
+  Γ ⊢ₛ e : τ → τ = τ' → Γ ⊢ₛ e : τ'.
+Proof. intros P eq. by simplify_eq. Qed.
 
 Reserved Notation "Γ & pΓ ⊢ₛ e : τ & pτ" (at level 74, pΓ, e, τ, pτ at next level).
 
-Inductive typed (Γ : list type) (pΓ : Forall TClosed Γ) : expr → forall (τ : type), TClosed τ → Prop :=
-  | Var_typed x τ pτ : (Γ !! x = Some τ) → Γ & pΓ ⊢ₛ Var x : τ & pτ
-  | Unit_typed pu : (Γ & pΓ ⊢ₛ Unit : TUnit & pu)
-  | Pair_typed e1 e2 τ1 pτ1 τ2 pτ2 pτ12 :
-      Γ & pΓ ⊢ₛ e1 : τ1&pτ1 →
-      Γ & pΓ ⊢ₛ e2 : τ2&pτ2 →
-      Γ & pΓ ⊢ₛ Pair e1 e2 : TProd τ1 τ2 & pτ12
-  | Fst_typed e τ1 pτ1 τ2 pτ12 :
-      Γ & pΓ ⊢ₛ e : TProd τ1 τ2 & pτ12 →
-      Γ & pΓ ⊢ₛ Fst e : τ1 & pτ1
-  | Snd_typed e τ1 τ2 pτ2 pτ12 :
-      Γ & pΓ ⊢ₛ e : TProd τ1 τ2 & pτ12 →
-      Γ & pΓ ⊢ₛ Snd e : τ2 & pτ2
-  | InjL_typed e τ1 pτ1 τ2 pτ12 :
-      Γ & pΓ ⊢ₛ e : τ1&pτ1 →
-      Γ & pΓ ⊢ₛ InjL e : TSum τ1 τ2 & pτ12
-  | InjR_typed e τ1 τ2 pτ2 pτ12 :
-      Γ & pΓ ⊢ₛ e : τ2 & pτ2 →
-      Γ & pΓ ⊢ₛ InjR e : TSum τ1 τ2 & pτ12
-  | Case_typed e0 e1 e2 τ1 pτ1 τ2 pτ2 pτ12 τ pτ :
-      Γ & pΓ ⊢ₛ e0 : TSum τ1 τ2 & pτ12 →
-      τ1 :: Γ & (Forall_cons _ _ _ pτ1 pΓ) ⊢ₛ e1 : τ & pτ →
-      τ2 :: Γ & (Forall_cons _ _ _ pτ2 pΓ) ⊢ₛ e2 : τ & pτ →
-      Γ & pΓ ⊢ₛ Case e0 e1 e2 : τ & pτ
-  | Lam_typed e τ1 pτ1 τ2 pτ2 pτ12 :
-      τ1 :: Γ & (Forall_cons _ _ _ pτ1 pΓ) ⊢ₛ e : τ2 & pτ2 →
-      Γ & pΓ ⊢ₛ Lam e : TArrow τ1 τ2 & pτ12
-  | App_typed e1 e2 τ1 pτ1 τ2 pτ2 pτ12 :
-      Γ & pΓ ⊢ₛ e1 : TArrow τ1 τ2 & pτ12 →
-      Γ & pΓ ⊢ₛ e2 : τ1 & pτ1 →
-      Γ & pΓ ⊢ₛ App e1 e2 : τ2 & pτ2
-  | Fold_typed e τb pτbμτb pμτb :
-      Γ & pΓ ⊢ₛ e : τb.[TRec τb/] & pτbμτb →
-      Γ & pΓ ⊢ₛ Fold e : TRec τb & pμτb
-  | Unfold_typed e τb pμτb pτbμτb :
-      Γ & pΓ ⊢ₛ e : TRec τb & pμτb →
-      Γ & pΓ ⊢ₛ Unfold e : τb.[TRec τb/] & pτbμτb
-where "Γ & pΓ ⊢ₛ e : τ & pτ" := (typed Γ pΓ e τ pτ).
-
-(* helper lemma's {{{ *)
-
-Lemma PI_typed Γ pΓ e τ pτ pτ' : Γ & pΓ ⊢ₛ e : τ & pτ → Γ & pΓ ⊢ₛ e : τ & pτ'.
-Proof. intro H. induction H; by econstructor. Qed.
-
-Lemma PI_Γ_typed Γ pΓ pΓ' e τ pτ : Γ & pΓ ⊢ₛ e : τ & pτ → Γ & pΓ' ⊢ₛ e : τ & pτ.
-Proof.
-  intro H. induction H; by econstructor.
-  Unshelve. auto. auto. auto.
-Qed.
-
-Lemma PI_Γ_typed' Γ pΓ' e τ pτ : forall pΓ, Γ & pΓ ⊢ₛ e : τ & pτ → Γ & pΓ' ⊢ₛ e : τ & pτ.
-Proof. intros pΓ H. by eapply PI_Γ_typed. Qed.
-
-Lemma Unfold_Fold_typed Γ pΓ e τ pτ :
-  Γ & pΓ ⊢ₛ e : τ & pτ → Γ & pΓ ⊢ₛ Unfold (Fold e) : τ & pτ.
-Proof.
-  intro.
-  assert (eq : τ = τ.[TRec τ/]). by rewrite pτ. generalize pτ. rewrite eq. intro pτμτ.
-  assert (pμτ : TClosed (TRec τ)). intro σ. asimpl. by rewrite pτ.
-  apply Unfold_typed with (pμτb := pμτ).
-  apply Fold_typed with (pτbμτb := pτμτ).
-  generalize pτμτ. rewrite -eq. intro pτ'.
-  by eapply PI_typed.
-Qed.
-
-Lemma Unfold_typed_help Γ pΓ e τb μτb τ' pτ' : (τb.[TRec τb/] = τ') →
-  Γ & pΓ ⊢ₛ e : (TRec τb) & μτb →
-  Γ & pΓ ⊢ₛ Unfold e : τ' & pτ'.
-Proof.
-  intros eq d.
-  generalize pτ'. rewrite -eq. intro pτ. eapply Unfold_typed.
-  by eapply PI_typed.
-  Unshelve. auto.
-Qed.
-
-Lemma rewrite_typed {Γ pΓ e τ pτ τ' pτ'} :
-  Γ & pΓ ⊢ₛ e : τ & pτ → τ = τ' → Γ & pΓ ⊢ₛ e : τ' & pτ'.
-Proof.
-  intros P eq.
-  generalize pτ'. rewrite -eq.
-  intro. by eapply PI_typed.
-Qed.
-
-(* }}} *)
-
 (* lemma's about substs in terms {{{ *)
 
-Lemma typed_subst_invariant Γ pΓ e τ pτ s1 s2 :
-  Γ & pΓ ⊢ₛ e : τ & pτ → (∀ x, x < length Γ → s1 x = s2 x) → e.[s1] = e.[s2].
+Lemma typed_subst_invariant Γ e τ s1 s2 :
+  Γ ⊢ₛ e : τ → (∀ x, x < length Γ → s1 x = s2 x) → e.[s1] = e.[s2].
 Proof.
   intros Htyped; revert s1 s2.
   assert (∀ x Γ, x < length (subst (ren (+1)) <$> Γ) → x < length Γ).
@@ -135,11 +95,27 @@ Proof.
     apply IHx.
 Qed.
 
-Lemma typed_n_closed Γ pΓ τ pτ e : Γ & pΓ ⊢ₛ e : τ & pτ → (∀ f, e.[upn (length Γ) f] = e).
+Lemma typed_n_closed Γ τ e : Γ ⊢ₛ e : τ → (∀ f, e.[upn (length Γ) f] = e).
 Proof.
   intros H. induction H => f; asimpl; simpl in *; auto with f_equal.
   apply lookup_lt_Some in H. rewrite iter_up. destruct lt_dec; auto with lia.
 Qed.
+
+Lemma Unfold_typed_help Γ e τ : (τ.[TRec τ/] = τ) → Γ ⊢ₛ e : TRec τ → Γ ⊢ₛ Unfold e : τ.
+Proof.
+  intros eq d.
+  rewrite -eq. by apply Unfold_typed.
+Qed.
+
+Lemma Unfold_typed_help_2 Γ e τ τ' : (τ.[TRec τ/] = τ') → Γ ⊢ₛ e : TRec τ → Γ ⊢ₛ Unfold e : τ'.
+Proof.
+  intros eq d.
+  rewrite -eq. by apply Unfold_typed.
+Qed.
+
+Definition Is_Closed τ := forall τ', τ.[τ'/] = τ.
+
+
 
 Lemma n_closed_invariant n (e : expr) s1 s2 :
   (∀ f, e.[upn n f] = e) → (∀ x, x < n → s1 x = s2 x) → e.[s1] = e.[s2].
@@ -175,62 +151,52 @@ Proof.
 Qed.
 
 (** Weakening *)
-Lemma context_gen_weakening ξ Γ' Γ α β e τ pτ :
-  Γ' ++ Γ & α ⊢ₛ e : τ & pτ →
-  Γ' ++ ξ ++ Γ & β ⊢ₛ e.[upn (length Γ') (ren (+ (length ξ)))] : τ & pτ.
+Lemma context_gen_weakening ξ Γ' Γ e τ :
+  Γ' ++ Γ ⊢ₛ e : τ →
+  Γ' ++ ξ ++ Γ ⊢ₛ e.[upn (length Γ') (ren (+ (length ξ)))] : τ.
 Proof.
   intros H1.
-  remember (Γ' ++ Γ) as Ξ. revert β. revert Γ' Γ ξ HeqΞ.
+  remember (Γ' ++ Γ) as Ξ. revert Γ' Γ ξ HeqΞ.
   induction H1 => Γ1 Γ2 ξ HeqΞ; subst; asimpl in *; eauto using typed.
   - rewrite iter_up; destruct lt_dec as [Hl | Hl].
-    + eapply Var_typed. rewrite lookup_app_l; trivial. by rewrite lookup_app_l in H.
-    + asimpl. eapply Var_typed. rewrite lookup_app_r; auto with lia.
+    + constructor. auto. rewrite lookup_app_l; trivial. by rewrite lookup_app_l in H.
+    + asimpl. constructor. auto. rewrite lookup_app_r; auto with lia.
       rewrite lookup_app_r; auto with lia.
       rewrite lookup_app_r in H; auto with lia.
       match goal with
         |- _ !! ?A = _ => by replace A with (x - length Γ1) by lia
       end.
   - econstructor; eauto. by apply (IHtyped2 (_::_)). by apply (IHtyped3 (_::_)).
-  - eapply Lam_typed. by apply (IHtyped (_ :: _)).
-    Unshelve. auto. auto. auto.
+  - constructor. auto. by apply (IHtyped (_ :: _)).
 Qed.
 
-Lemma context_weakening ξ Γ pΓ α e τ pτ :
-  Γ & pΓ ⊢ₛ e : τ & pτ → ξ ++ Γ & α ⊢ₛ e.[(ren (+ (length ξ)))] : τ & pτ.
+Lemma context_weakening ξ Γ e τ :
+  Γ ⊢ₛ e : τ → ξ ++ Γ ⊢ₛ e.[(ren (+ (length ξ)))] : τ.
 Proof. eapply (context_gen_weakening _ []). Qed.
 
-Lemma up_type i Γ pΓ e τ pτ Γ' α : (length Γ' = i) -> (Γ & pΓ ⊢ₛ e : τ & pτ) -> (Γ' ++ Γ) & α ⊢ₛ e.[ren (+i)] : τ & pτ.
-Proof.
-  intros.
-  simplify_eq.
-  by eapply context_weakening.
-Qed.
+(* Lemma context_gen_reorder Γ'' Γ' Γ τ1 τ2 τe τ : *)
+  (* Γ'' ++ [τ1] ++ Γ' ++ [τ2] ++ Γ ⊢ₛ e : τ → *)
+  (* Γ'' ++ [τ2] ++ Γ' ++ [τ1] ++ Γ' ⊢ₛ e.[upn (length Γ') (ren (+ (length ξ)))] : τ. *)
 
-Lemma up_type_one Γ pΓ e τ pτ τ' pτ' :
-  (Γ & pΓ ⊢ₛ e : τ & pτ) ->
-  ((τ' :: Γ) & (List.Forall_cons TClosed _ _ pτ' pΓ) ⊢ₛ e.[ren (+1)] : τ & pτ).
-Proof.
-  intro.
-  assert (T : τ' :: Γ = [τ'] ++ Γ). done. generalize (Forall_cons TClosed τ' Γ pτ' pΓ). rewrite T. intro α'.
-  by eapply up_type.
-Qed.
+Lemma closed_context_weakening ξ Γ e τ :
+  (∀ f, e.[f] = e) → Γ ⊢ₛ e : τ → ξ ++ Γ ⊢ₛ e : τ.
+Proof. intros H1 H2. erewrite <- H1. by eapply context_weakening. Qed.
 
-Lemma up_type_two Γ pΓ e τ pτ τ' τ'' α :
-  (Γ & pΓ ⊢ₛ e : τ & pτ) ->
-  τ' :: τ'' :: Γ & α ⊢ₛ e.[ren (+2)] : τ & pτ.
-Proof.
-  intros.
-  assert (T : τ' :: τ'' :: Γ = [τ' ; τ''] ++ Γ). done. generalize α. rewrite T. intro.
-  by eapply up_type.
-Qed.
+Lemma up_type i Γ e τ Γ' : (length Γ' = i) -> (Γ ⊢ₛ e : τ) -> (Γ' ++ Γ) ⊢ₛ e.[ren (+i)] : τ.
+Proof. intros. simplify_eq. by apply context_weakening. Qed.
 
-Lemma EClosed_typed e τ pτ :
-  EClosed e → ([] & (Forall_nil TClosed) ⊢ₛ e : τ & pτ) → forall Γ pΓ, Γ & pΓ ⊢ₛ e : τ & pτ.
+Lemma up_type_one Γ e τ τ' : (Γ ⊢ₛ e : τ) -> τ' :: Γ ⊢ₛ e.[ren (+1)] : τ.
+Proof. intro. assert (T : τ' :: Γ = [τ'] ++ Γ). done. rewrite T. by apply up_type. Qed.
+
+Lemma up_type_two Γ e τ τ' τ'' : (Γ ⊢ₛ e : τ) -> τ' :: τ'' :: Γ ⊢ₛ e.[ren (+2)] : τ.
+Proof. intros. assert (T : τ' :: τ'' :: Γ = [τ' ; τ''] ++ Γ). done. rewrite T. by apply up_type. Qed.
+
+Lemma EClosed_typed e τ :
+  EClosed e → ([] ⊢ₛ e : τ) → forall Γ, (Γ ⊢ₛ e : τ).
 Proof.
-  intros pe H Γ pΓ.
-  cut (forall α, Γ ++ [] & α ⊢ₛ e.[(ren (+ (length Γ)))]: τ & pτ).
-  by rewrite app_nil_r pe. intro. eapply context_weakening.
-  apply H.
+  intros ec H Γ.
+  cut (Γ ++ [] ⊢ₛ e.[(ren (+ (length Γ)))]: τ).
+  rewrite app_nil_r. by rewrite ec. by eapply context_weakening.
 Qed.
 
 (* }}} *)
