theories/backtranslation/cast_help/factorize.v
@@ -7,11 +7,10 @@ From fae_gtlc_mu.backtranslation.cast_help Require Export universe embed extract
 Definition identity : val :=
   LamV (Var 0).
 
-Lemma identity_typed Γ pΓ τ pτ : Γ & pΓ ⊢ₛ identity : (TArrow τ τ) & (TArrow_closed pτ pτ).
+Lemma identity_typed Γ τ (pτ : TClosed τ) : Γ ⊢ₛ identity : (TArrow τ τ).
 Proof.
   intros.
-  eapply Lam_typed. by apply Var_typed.
-  Unshelve. all:auto.
+  eapply Lam_typed; auto. by apply Var_typed.
 Qed.
 
 (** Factorisations *)
@@ -24,64 +23,17 @@ Definition factorization (f g : expr) : val :=
 Lemma factorization_subst_rewrite (f g : expr) σ : (# (factorization f g)).[σ] = factorization f.[σ] g.[σ].
 Proof. by asimpl. Qed.
 
-Lemma factorization_typed Γ pΓ {f g : expr} (τ1 : type) pτ1 τ2 pτ2 τ3 pτ3
-      (df : Γ & pΓ ⊢ₛ f : (TArrow τ1 τ2) & TArrow_closed pτ1 pτ2)
-      (dg : Γ & pΓ ⊢ₛ g : (TArrow τ2 τ3) & TArrow_closed pτ2 pτ3) :
-  Γ & pΓ ⊢ₛ factorization f g : (TArrow τ1 τ3) & TArrow_closed pτ1 pτ3.
+Lemma factorization_typed Γ {f g : expr} τ1 τ2 τ3
+      (df : Γ ⊢ₛ f : TArrow τ1 τ2)
+      (dg : Γ ⊢ₛ g : TArrow τ2 τ3) :
+  Γ ⊢ₛ factorization f g : TArrow τ1 τ3.
 Proof.
-  eapply Lam_typed.
-  eapply App_typed with (τ1 := τ2).
-  eapply up_type_one. apply dg.
-  eapply App_typed with (τ1 := τ1).
-  eapply up_type_one. apply df.
-  by apply Var_typed.
-  Unshelve. all:auto.
+  apply Lam_typed; auto.
+  apply (TArrow_closed1 (typed_closed df)).
+  apply App_typed with (τ1 := τ2).
+  apply up_type_one. apply dg.
+  apply App_typed with (τ1 := τ1).
+  apply up_type_one. apply df.
+  apply Var_typed; auto.
+  apply (TArrow_closed1 (typed_closed df)).
 Qed.
-
-(* Definition factorization_up (f : expr) (τG : cast_calculus.types.type) (G : Ground τG) : val := *)
-(*   LamV ( *)
-(*       embed τG G (f.[ren (+1)] (Var 0)) *)
-(*     ). *)
-
-(* Lemma factorization_up_subst_rewrite (f : expr) (τG : cast_calculus.types.type) (G : Ground τG) σ : (# (factorization_up f τG G)).[σ] = factorization_up f.[σ] τG G. *)
-(* Proof. *)
-(*   rewrite /factorization_up. *)
-(*   asimpl. by rewrite embed_no_subs. *)
-(* Qed. *)
-
-(* Lemma factorization_up_typed Γ pΓ {f : expr} (τ : type) pτ (τG : cast_calculus.types.type) (G : Ground τG) *)
-(*       (d : Γ & pΓ ⊢ₛ f : (TArrow τ <<τG>>) & TArrow_closed pτ (back_Ground_closed G)) : *)
-(*   Γ & pΓ ⊢ₛ factorization_up f τG G : (TArrow τ Universe) & TArrow_closed pτ Universe_closed. *)
-(* Proof. *)
-(*   eapply Lam_typed. *)
-(*   eapply App_typed with (τ1 := << τG >>). *)
-(*   apply embed_typed. *)
-(*   eapply App_typed with (τ1 := τ ). *)
-(*   eapply up_type_one. apply d. *)
-(*   by apply Var_typed. *)
-(*   Unshelve. all:(auto||apply Universe_closed||by apply back_Ground_closed). *)
-(* Qed. *)
-
-(* Definition factorization_down (f : expr) (τG : cast_calculus.types.type) (G : Ground τG) : val := *)
-(*   LamV ( *)
-(*       (f.[ren (+1)]) (extract τG G (Var 0)) *)
-(*     ). *)
-
-(* Lemma factorization_down_subst_rewrite (f : expr) (τG : cast_calculus.types.type) (G : Ground τG) σ : (# (factorization_down f τG G)).[σ] = factorization_down f.[σ] τG G. *)
-(* Proof. *)
-(*   rewrite /factorization_down. *)
-(*   asimpl. by rewrite extract_no_subs. *)
-(* Qed. *)
-
-(* Lemma factorization_down_typed Γ pΓ {f : expr} (τ : type) pτ (τG : cast_calculus.types.type) (G : Ground τG) *)
-(*       (d : Γ & pΓ ⊢ₛ f : (TArrow <<τG>> τ) & (TArrow_closed (back_Ground_closed G) pτ)) : *)
-(*   Γ & pΓ ⊢ₛ factorization_down f τG G : (TArrow Universe τ) & (TArrow_closed Universe_closed pτ). *)
-(* Proof. *)
-(*   eapply Lam_typed. *)
-(*   eapply App_typed with (τ1 := << τG >>). *)
-(*   eapply up_type_one. apply d. *)
-(*   eapply App_typed with (τ1 := Universe). *)
-(*   apply extract_typed. *)
-(*   by apply Var_typed. *)
-(*   Unshelve. all:(auto||apply Universe_closed||by apply back_Ground_closed). *)
-(* Qed. *)
