theories/backtranslation/cast_help/props/extract_embed.v
@@ -1,0 +1,81 @@
+From fae_gtlc_mu.stlc_mu Require Export lang.
+From fae_gtlc_mu.backtranslation.cast_help Require Export extract embed.
+
+(* from resourcers_left {{{ *)
+
+(* From fae_gtlc_mu.refinements.static_gradual Require Export resources_left. *)
+
+Ltac inv_head_step :=
+  repeat match goal with
+  (* | _ => progress simplify_map_eq/= (* simplify memory stuff *) *)
+  | H : to_val _ = Some _ |- _ => apply of_to_val in H
+  | H : head_step ?e _ _ _ _ _ |- _ =>
+      try (is_var e; fail 1); (* inversion yields many goals if [e] is a variable
+      and can thus better be avoided. *)
+      inversion H; subst; clear H
+  end.
+
+Local Ltac solve_exec_safe := intros; subst; do 3 eexists; econstructor; eauto.
+Local Ltac solve_exec_puredet := simpl; intros; by inv_head_step.
+Local Ltac solve_pure_exec :=
+  unfold IntoVal in *;
+  repeat match goal with H : AsVal _ |- _ => destruct H as [??] end; subst;
+  intros ?; apply nsteps_once, pure_head_step_pure_step;
+    constructor; [solve_exec_safe | solve_exec_puredet].
+
+(* }}} *)
+
+Ltac ps_head_step := apply pure_head_step_pure_step;
+    constructor; [solve_exec_safe | solve_exec_puredet]; try (by rewrite /= to_of_val /=).
+
+Ltac new_step := eapply nsteps_l.
+
+Lemma extract_TUnit_embed_TUnit v : nsteps pure_step 6 (extract_TUnit (embedV_TUnit v)) v.
+Proof.
+  new_step. ps_head_step.
+  new_step. apply (pure_step_ctx (fill_item (CaseCtx _ _))). ps_head_step. simpl.
+  new_step. ps_head_step.
+  new_step. ps_head_step.
+  new_step. ps_head_step.
+  new_step. ps_head_step.
+  constructor.
+Qed.
+
+Lemma extract_TProd_embed_TProd v : nsteps pure_step 5 (extract_Ground_TProd (embedV_Ground_TProd v)) v.
+Proof.
+  new_step. ps_head_step.
+  new_step. apply (pure_step_ctx (fill_item (CaseCtx _ _))). ps_head_step. simpl.
+  new_step. ps_head_step.
+  new_step. ps_head_step.
+  new_step. ps_head_step.
+  constructor.
+Qed.
+
+Lemma extract_TArrow_embed_TArrow v : nsteps pure_step 4 (extract_Ground_TArrow (embedV_Ground_TArrow v)) v.
+Proof.
+  new_step. ps_head_step.
+  new_step. apply (pure_step_ctx (fill_item (CaseCtx _ _))). ps_head_step. simpl.
+  new_step. ps_head_step.
+  new_step. ps_head_step.
+  constructor.
+Qed.
+
+Lemma extract_TSum_embed_TSum v : nsteps pure_step 6 (extract_Ground_TSum (embedV_Ground_TSum v)) v.
+Proof.
+  new_step. ps_head_step.
+  new_step. apply (pure_step_ctx (fill_item (CaseCtx _ _))). ps_head_step. simpl.
+  new_step. ps_head_step.
+  new_step. ps_head_step.
+  new_step. ps_head_step.
+  new_step. ps_head_step.
+  constructor.
+Qed.
+
+
+Lemma extract_TRec_embed_TUnknown v : nsteps pure_step 3 (extract_Ground_TRec (# embedV_TUnknown v)) (Fold (# v)).
+Proof.
+  new_step. ps_head_step.
+  new_step. apply (pure_step_ctx (fill_item (CaseCtx _ _))). ps_head_step. simpl.
+  new_step. ps_head_step.
+  constructor.
+Qed.
