theories/backtranslation/well_typedness.v
@@ -1,89 +1,67 @@
-From fae_gtlc_mu.cast_calculus Require Export typing (*contexts*).
-From fae_gtlc_mu.stlc_mu Require Export typing (*contexts*).
+From fae_gtlc_mu.cast_calculus Require Export typing contexts.
+From fae_gtlc_mu.stlc_mu Require Export typing contexts.
 
-From fae_gtlc_mu.backtranslation Require Import types expressions cast_help.general (*contexts*).
+From fae_gtlc_mu.backtranslation Require Import types expressions cast_help.general contexts.
 
-Lemma force_typed Γ Γ' pΓ pΓ' e τ τ' pτ pτ' : Γ & pΓ ⊢ₛ e : τ & pτ → Γ = Γ' → τ = τ' → Γ' & pΓ' ⊢ₛ e : τ & pτ'. (** use with cae *)
-Proof. intros. simplify_eq. eapply PI_typed. eapply PI_Γ_typed. done. Qed.
-
-Lemma well_typedness_expr Γ pΓ e τ pτ :
-  Γ & pΓ ⊢ₜ e : τ & pτ →
-    map backtranslate_type Γ & (Forall_fmap_impl _ _ _ _ (@back_closed) pΓ) ⊢ₛ backtranslate_expr e : backtranslate_type τ & (back_closed pτ).
+Lemma well_typedness_expr Γ e τ : (Γ ⊢ₜ e : τ) →
+    map backtranslate_type Γ ⊢ₛ backtranslate_expr e : backtranslate_type τ.
 Proof.
   induction 1; simpl; try by econstructor.
-  - constructor. by rewrite list_lookup_fmap H.
-  - eapply Case_typed. apply IHtyped1.
-    eapply PI_typed. eapply PI_Γ_typed. apply IHtyped2.
-    eapply PI_typed. eapply PI_Γ_typed. apply IHtyped3.
-  - eapply Lam_typed. eapply PI_Γ_typed. apply IHtyped.
-  - assert (HC : TClosed <<(τb.[cast_calculus.types.TRec τb/])>>). by apply back_closed.
-    eapply rewrite_typed.
-    eapply Fold_typed. eapply PI_Γ_typed. eapply rewrite_typed. apply IHtyped.
-    rewrite back_unfold_comm. auto. auto.
-  - eapply Unfold_typed_help. by rewrite back_unfold_comm.
-    eapply rewrite_typed. by apply IHtyped. by simpl.
-  - destruct (decide (cons_stand_open τi τf)); destruct (decide (cast_calculus.types.TClosed τi)); destruct (decide (cast_calculus.types.TClosed τf)); try by contradiction.
-    eapply App_typed.
-    apply EClosed_typed. apply 𝓕c_closed; auto.
-    rewrite /𝓕c /env_subst. asimpl. eapply force_typed. apply 𝓕_typed. auto. auto.
-    apply IHtyped.
-  - apply Ω_typed.
-  Unshelve.
-   try by apply back_closed.
-   try by apply back_closed.
-   try by apply back_closed.
-   cut (TClosed (<<(cast_calculus.types.TRec τb)>>)). by simpl.
-   by apply back_closed.
-   by rewrite back_unfold_comm in HC.
-   cut (TClosed (<<(cast_calculus.types.TRec τb)>>)). by simpl.
-   by apply back_closed.
-   cut (TClosed (<<(cast_calculus.types.TArrow τi τf)>>)). by simpl.
-   apply back_closed. by apply cast_calculus.types.TArrow_closed.
-   auto.
-   auto.
-   auto.
+  - constructor. by apply back_closed. by rewrite list_lookup_fmap H.
+  - apply InjL_typed. by apply back_closed. auto.
+  - apply InjR_typed. by apply back_closed. auto.
+  - eapply Lam_typed. by apply back_closed. apply IHtyped.
+  - apply Fold_typed.
+    by rewrite back_unfold_comm in IHtyped.
+  - rewrite back_unfold_comm.
+    by apply Unfold_typed.
+  - assert (pτi : cast_calculus.types.TClosed τi). apply (cast_calculus.typing.typed_closed H).
+    destruct (cons_stand_open_dec τi τf);
+      destruct (decide (cast_calculus.types.TClosed τi));
+      destruct (decide (cast_calculus.types.TClosed τf)); try by contradiction.
+    eapply App_typed with (τ1 := <<τi>>).
+    apply EClosed_typed; auto. apply 𝓕c_closed; auto.
+    rewrite /𝓕c /env_subst. asimpl.
+    apply 𝓕_typed with (A := []); auto. apply IHtyped.
+  - apply Ω_typed. by apply back_closed.
 Qed.
 
 (* From fae_gtlc_mu.embedding Require Export types. *)
 
-(* Lemma well_typedness_ctx_item Γ τ Γ' τ' C : *)
-(*   cast_calculus.contexts.typed_ctx_item C Γ τ Γ' τ' → *)
-(*   typed_ctx_item (backtranslate_ctx_item C) (map backtranslate_type Γ) (backtranslate_type τ) (map backtranslate_type Γ') (backtranslate_type τ'). *)
-(* Proof. *)
-(*   induction 1; try (by constructor). *)
-(*   - apply TP_CTX_AppL. apply well_typedness_expr; done. *)
-(*   - apply TP_CTX_AppR. *)
-(*     assert (triv : backtranslate_type (types.TArrow τ τ') = TArrow <<τ>> <<τ'>>). by simpl. rewrite -triv. clear triv. *)
-(*     by apply well_typedness_expr. *)
-(*   - constructor. by apply well_typedness_expr. *)
-(*   - constructor. by apply well_typedness_expr. *)
-(*   - constructor. *)
-(*     assert (triv : backtranslate_type τ1 :: (map backtranslate_type Γ) = map backtranslate_type (τ1 :: Γ)). by simpl. rewrite triv. clear triv. *)
-(*       by apply well_typedness_expr. *)
-(*     assert (triv : backtranslate_type τ2 :: (map backtranslate_type Γ) = map backtranslate_type (τ2 :: Γ)). by simpl. rewrite triv. clear triv. *)
-(*       by apply well_typedness_expr. *)
-(*   - apply TP_CTX_CaseM with (τ2 := <<τ2>>). *)
-(*     assert (triv : backtranslate_type (types.TSum τ1 τ2) = TSum <<τ1>> <<τ2>>). by simpl. rewrite -triv. clear triv. *)
-(*       by apply well_typedness_expr. *)
-(*     assert (triv : backtranslate_type τ2 :: (map backtranslate_type Γ) = map backtranslate_type (τ2 :: Γ)). by simpl. rewrite triv. clear triv. *)
-(*       by apply well_typedness_expr. *)
-(*   - apply TP_CTX_CaseR with (τ1 := <<τ1>>). *)
-(*     assert (triv : backtranslate_type (types.TSum τ1 τ2) = TSum <<τ1>> <<τ2>>). by simpl. rewrite -triv. clear triv. *)
-(*       by apply well_typedness_expr. *)
-(*     assert (triv : backtranslate_type τ1 :: (map backtranslate_type Γ) = map backtranslate_type (τ1 :: Γ)). by simpl. rewrite triv. clear triv. *)
-(*       by apply well_typedness_expr. *)
-(*   - rewrite back_unfold_comm. apply TP_CTX_Fold. *)
-(*   - rewrite back_unfold_comm. apply TP_CTX_Unfold. *)
-(*   - simpl. destruct (cons_stand_dec τi τf); destruct (decide (TClosed τi)); destruct (decide (TClosed τf)); try by contradiction. *)
-(*     eapply TP_CTX_AppR. admit. *)
-(* Admitted. *)
+Lemma well_typedness_ctx_item Γ τ (pτ : cast_calculus.types.TClosed τ) Γ' τ' C :
+  cast_calculus.contexts.typed_ctx_item C Γ τ Γ' τ' →
+  typed_ctx_item (backtranslate_ctx_item C) (map backtranslate_type Γ) (backtranslate_type τ) (map backtranslate_type Γ') (backtranslate_type τ').
+Proof.
+  induction 1; try (by constructor).
+  - apply TP_CTX_Lam. by apply back_closed.
+  - apply TP_CTX_AppL. apply well_typedness_expr; done.
+  - apply TP_CTX_AppR.
+    cut (map backtranslate_type Γ ⊢ₛ backtranslate_expr e1 : <<(cast_calculus.types.TArrow τ τ')>>). by simpl.
+    by apply well_typedness_expr.
+  - constructor. by apply well_typedness_expr.
+  - constructor. by apply well_typedness_expr.
+  - constructor. by apply back_closed.
+  - constructor. by apply back_closed.
+  - constructor; rewrite -map_cons; by apply well_typedness_expr.
+  - eapply TP_CTX_CaseM with (τ2 := <<τ2>>); auto.
+    cut (map backtranslate_type Γ ⊢ₛ backtranslate_expr e0 : <<(cast_calculus.types.TSum τ1 τ2)>>). by simpl.
+    by apply well_typedness_expr. rewrite -map_cons. by apply well_typedness_expr.
+  - eapply TP_CTX_CaseR with (τ1 := <<τ1>>); auto.
+    cut (map backtranslate_type Γ ⊢ₛ backtranslate_expr e0 : <<(cast_calculus.types.TSum τ1 τ2)>>). by simpl.
+    by apply well_typedness_expr. rewrite -map_cons. by apply well_typedness_expr.
+  - rewrite back_unfold_comm. apply TP_CTX_Fold.
+  - rewrite back_unfold_comm. apply TP_CTX_Unfold.
+  - simpl. destruct (cons_stand_open_dec τi τf); destruct (decide (cast_calculus.types.TClosed τi)); destruct (decide (cast_calculus.types.TClosed τf)); try by contradiction.
+    apply TP_CTX_AppR. apply EClosed_typed. apply 𝓕c_closed; auto.
+    rewrite /𝓕c /=. asimpl. apply 𝓕_typed with (A := []); auto.
+Qed.
 
-(* Lemma well_typedness_ctx Γ τ Γ' τ' C : *)
-(*   cast_calculus.contexts.typed_ctx C Γ τ Γ' τ' → *)
-(*   typed_ctx (backtranslate_ctx C) (map backtranslate_type Γ) (backtranslate_type τ) (map backtranslate_type Γ') (backtranslate_type τ'). *)
-(* Proof. *)
-(*   induction 1. *)
-(*   - constructor. *)
-(*   - econstructor; simpl. by apply well_typedness_ctx_item. *)
-(*     auto. *)
-(* Qed. *)
+Lemma well_typedness_ctx Γ τ (pτ : cast_calculus.types.TClosed τ) Γ' τ' C :
+  cast_calculus.contexts.typed_ctx C Γ τ Γ' τ' →
+  typed_ctx (backtranslate_ctx C) (map backtranslate_type Γ) (backtranslate_type τ) (map backtranslate_type Γ') (backtranslate_type τ').
+Proof.
+  induction 1.
+  - constructor.
+  - econstructor; simpl. apply well_typedness_ctx_item with (τ := τ2).
+    eapply cast_calculus.contexts.typed_ctx_closedness. apply pτ. apply H0. apply H. apply IHtyped_ctx. auto.
+Qed.
