theories/cast_calculus/consistency/equivalence/first_half.v
@@ -1,0 +1,229 @@
+From stdpp Require Import base list.
+From Autosubst Require Export Autosubst.
+Require Export Utf8_core.
+From fae_gtlc_mu.cast_calculus Require Import types consistency.standard consistency.equivalence.intermediate upper_bound.
+Require Import Relation_Operators.
+Require Import Transitive_Closure.
+From Coq.Wellfounded Require Import Lexicographic_Product Union.
+From Coq.Program Require Import Wf.
+
+
+Lemma smart_lookup (l : list (type * type)) (x : type * type) : (sum { i : nat & l !! i = Some x } (x ∉ l)).
+Proof.
+  destruct (decide (x ∈ l)).
+  - left.
+    induction l.
+    + exfalso. inversion e.
+    + destruct (decide (x = a)).
+      * rewrite e0. by exists 0.
+      * destruct (decide (x ∈ l)).
+        destruct (IHl e0). exists (S x0). by simpl.
+        exfalso. inversion e. simplify_eq. by apply n0.
+  - by right.
+Qed.
+
+Definition lexord : relation (@sigT nat (fun _ => nat)) :=
+  (lexprod _ _ lt (fun _ => lt)).
+
+Lemma ord_left n n' m m' : n < n' → lexord (existT n m) (existT n' m').
+Proof.
+  intros. by apply left_lex.
+Qed.
+
+Lemma ord_right n n' m m' : n ≤ n' → m < m' → lexord (existT n m) (existT n' m').
+Proof.
+  intros.
+  destruct (decide (n < n')).
+  - by apply left_lex.
+  - assert (triv : n = n'). lia. rewrite triv. clear triv.
+    by apply right_lex.
+Qed.
+
+Fixpoint size (τ : type) : nat :=
+  match τ with
+  | TUnit => 1
+  | TProd τ1 τ2 => size τ1 + size τ2
+  | TSum τ1 τ2 => size τ1 + size τ2
+  | TArrow τ1 τ2 => size τ1 + size τ2
+  | TRec τ => S (size τ)
+  | TVar x => 1
+  | TUnknown => 1
+  end.
+
+Lemma size_gt_0 τ : 0 < size τ.
+Proof. induction τ; simpl; lia. Qed.
+
+Definition size_pair (p : type * type) : nat :=
+  match p with | pair x x0 => size x + size x0 end.
+
+Require Import JMeq.
+
+(** TODO; remove program fixpoint... *)
+
+(* Lemma struct_validity (A : list (type * type)) (pA : Forall (fun p => TClosed p.1 ∧ TClosed p.2) A) *)
+(*       τ (pτC : TClosed τ) τ' (pτ'C : TClosed τ') (pStand : cons_stand τ τ') : cons_struct_pre A τ τ'. *)
+(* Proof. *)
+
+Inductive Cat : type → Type :=
+  | CUnknown : Cat TUnknown
+  | CGroundUnit : Ground TUnit → Cat TUnit
+  | CGroundProd : Ground (TProd TUnknown TUnknown) → Cat (TProd TUnknown TUnknown)
+  | CGroundSum : Ground (TSum TUnknown TUnknown) → Cat (TSum TUnknown TUnknown)
+  | CGroundArrow : Ground (TArrow TUnknown TUnknown) → Cat (TArrow TUnknown TUnknown)
+  | CGroundRec : Ground (TRec TUnknown) → Cat (TRec TUnknown)
+  | CProd τ1 τ2 : (τ1 ≠ TUnknown ∨ τ2 ≠ TUnknown) → Cat (TProd τ1 τ2)
+  | CSum τ1 τ2 : (τ1 ≠ TUnknown ∨ τ2 ≠ TUnknown) → Cat (TSum τ1 τ2)
+  | CArrow τ1 τ2 : (τ1 ≠ TUnknown ∨ τ2 ≠ TUnknown) → Cat (TArrow τ1 τ2)
+  | CRec τ : (τ ≠ TUnknown) → Cat (TRec τ)
+  | CVar i : Cat (TVar i).
+
+Lemma categorize (τ : type) : Cat τ.
+Proof.
+  destruct τ; try by do 2 constructor.
+  - destruct (decide (τ1 = ⋆)); simplify_eq.
+    destruct (decide (τ2 = ⋆)); simplify_eq.
+    constructor. constructor. constructor; auto. constructor; auto.
+  - destruct (decide (τ1 = ⋆)); simplify_eq.
+    destruct (decide (τ2 = ⋆)); simplify_eq.
+    constructor. constructor. constructor; auto. constructor; auto.
+  - destruct (decide (τ1 = ⋆)); simplify_eq.
+    destruct (decide (τ2 = ⋆)); simplify_eq.
+    constructor. constructor. constructor; auto. constructor; auto.
+  - destruct (decide (τ = ⋆)); simplify_eq.
+    constructor. constructor. constructor; auto.
+Qed.
+
+
+Program Fixpoint struct_validity (A : list (type * type)) (pA : Forall (fun p => TClosed p.1 ∧ TClosed p.2) A) τ (pτC : TClosed τ) τ' (pτ'C : TClosed τ') (pStand : cons_stand_open τ τ')
+        {measure (existT (upper_bound A τ τ') (size_pair (τ , τ'))) lexord} : cons_struct_pre A τ τ' :=
+  match pStand with
+  | GenSymUnit => consp_BaseBase A
+  | GenSymUnknownL τr => _
+  | GenSymUnknownR τl => _
+  | GenSymProd τ1 τ1' τ2 τ2' s1 s2 =>
+    consp_TProdTProd A τ1 τ1' τ2 τ2'
+                     (struct_validity A pA τ1 ltac:(simplify_eq; by apply (TProd_closed1 pτC)) τ1' ltac:(simplify_eq; by apply (TProd_closed1 pτ'C)) s1)
+                     (struct_validity A pA τ2 ltac:(simplify_eq; by apply (TProd_closed2 pτC)) τ2' ltac:(simplify_eq; by apply (TProd_closed2 pτ'C)) s2)
+  | GenSymSum τ1 τ1' τ2 τ2' s1 s2 =>
+    consp_TSumTSum A τ1 τ1' τ2 τ2'
+                     (struct_validity A pA τ1 ltac:(simplify_eq; by apply (TSum_closed1 pτC)) τ1' ltac:(simplify_eq; by apply (TSum_closed1 pτ'C)) s1)
+                     (struct_validity A pA τ2 ltac:(simplify_eq; by apply (TSum_closed2 pτC)) τ2' ltac:(simplify_eq; by apply (TSum_closed2 pτ'C)) s2)
+  | GenSymArrow τ1 τ1' τ2 τ2' s1 s2 =>
+    consp_TArrowTArrow A τ1 τ1' τ2 τ2'
+                     (struct_validity A pA τ1' ltac:(simplify_eq; by apply (TArrow_closed1 pτ'C)) τ1 ltac:(simplify_eq; by apply (TArrow_closed1 pτC)) (cons_stand_open_sym s1))
+                     (struct_validity A pA τ2 ltac:(simplify_eq; by apply (TArrow_closed2 pτC)) τ2' ltac:(simplify_eq; by apply (TArrow_closed2 pτ'C)) s2)
+  | GenSymVar i => ltac:(simplify_eq; exfalso; apply (no_var_is_closed i pτC))
+  | GenSymRec τ τ' P => _
+    (* match decide (exists (i : nat), A !! i = Some (TRec τ , TRec τ')) with *)
+    (* | left pYes => consTRecTRecUseCall A τ τ' _ _ *)
+    (* | right pNo => consTRecTRecExposeCall A τ τ' _ (struct_validity ((TRec τ, TRec τ') :: A) τ.[TRec τ/] ltac:(simplify_eq; by apply (TRec_closed_unfold pτC)) τ'.[TRec τ'/] ltac:(simplify_eq; by apply (TRec_closed_unfold pτ'C)) (cons_stand_unfold P)) *)
+    (* end *)
+  end.
+
+Next Obligation.
+Proof.
+  intros; simplify_eq.
+  destruct (categorize τ'); (try (by apply consp_StarTGround)); try apply consp_StarStar.
+  - apply consp_GroundProdTau; auto.
+    apply (struct_validity A pA TUnknown pτC τ1 (TProd_closed1 pτ'C) (GenSymUnknownL τ1)).
+    { simpl. apply ord_right. apply upper_bound_le_unknown_prod1. pose (p := size_gt_0 τ2). lia. }
+    apply (struct_validity A pA TUnknown pτC τ2 (TProd_closed2 pτ'C) (GenSymUnknownL τ2)).
+    { simpl. apply ord_right. apply upper_bound_le_unknown_prod2. pose (p := size_gt_0 τ1). lia. }
+  - apply consp_GroundSumTau; auto.
+    apply (struct_validity A pA TUnknown pτC τ1 (TSum_closed1 pτ'C) (GenSymUnknownL τ1)).
+    { simpl. apply ord_right. apply upper_bound_le_unknown_sum1. pose (p := size_gt_0 τ2). lia. }
+    apply (struct_validity A pA TUnknown pτC τ2 (TSum_closed2 pτ'C) (GenSymUnknownL τ2)).
+    { simpl. apply ord_right. apply upper_bound_le_unknown_sum2. pose (p := size_gt_0 τ1). lia. }
+  - apply consp_GroundArrowTau; auto.
+    apply (struct_validity A pA τ1 (TArrow_closed1 pτ'C) TUnknown pτC (GenSymUnknownR τ1)).
+    { simpl. apply ord_right. apply upper_bound_le_unknown_arrow_con. pose (p := size_gt_0 τ2). lia. }
+    apply (struct_validity A pA TUnknown pτC τ2 (TArrow_closed2 pτ'C) (GenSymUnknownL τ2)).
+    { simpl. apply ord_right. apply upper_bound_le_unknown_arrow_cov.  pose (p := size_gt_0 τ1). lia. }
+  - destruct (smart_lookup A (TRec TUnknown , TRec τ)) as [[i p] | np].
+    + by apply (consp_GroundRecTauUseCall A τ i).
+    + apply consp_GroundRecTauExposeCall; auto.
+      apply (struct_validity ((TRec TUnknown, TRec τ) :: A)). constructor; simpl; auto. split; auto. done. done. apply (TRec_closed_unfold pτ'C).
+      assert (H : TUnknown = TUnknown.[TRec TUnknown/]). by asimpl. rewrite H.
+      apply GenSymUnknownL.
+      { simpl. apply ord_left. apply upper_bound_lt_star_rec; auto. }
+  - exfalso. apply (no_var_is_closed i pτ'C).
+Qed.
+
+Next Obligation.
+  intros; simplify_eq.
+  destruct (categorize τ); (try (by apply consp_TGroundStar)); try apply consp_StarStar.
+  - apply consp_TauGroundProd; auto.
+    apply (struct_validity A pA τ1 (TProd_closed1 pτC) TUnknown pτ'C (GenSymUnknownR τ1)).
+    { simpl. apply ord_right. apply upper_bound_le_prod_unknown1. pose (p := size_gt_0 τ2). lia. }
+    apply (struct_validity A pA τ2 (TProd_closed2 pτC) TUnknown pτ'C (GenSymUnknownR τ2)).
+    { simpl. apply ord_right. apply upper_bound_le_prod_unknown2. pose (p := size_gt_0 τ1). lia. }
+  - apply consp_TauGroundSum; auto.
+    apply (struct_validity A pA τ1 (TSum_closed1 pτC) TUnknown pτ'C (GenSymUnknownR τ1)).
+    { simpl. apply ord_right. apply upper_bound_le_sum_unknown1. pose (p := size_gt_0 τ2). lia. }
+    apply (struct_validity A pA τ2 (TSum_closed2 pτC) TUnknown pτ'C (GenSymUnknownR τ2)).
+    { simpl. apply ord_right. apply upper_bound_le_sum_unknown2. pose (p := size_gt_0 τ1). lia. }
+  - apply consp_TauGroundArrow; auto.
+    apply (struct_validity A pA TUnknown pτ'C τ1 (TArrow_closed1 pτC) (GenSymUnknownL τ1)).
+    { simpl. apply ord_right. apply upper_bound_le_arrow_unknown_con. pose (p := size_gt_0 τ2). lia. }
+    apply (struct_validity A pA τ2 (TArrow_closed2 pτC) TUnknown pτ'C (GenSymUnknownR τ2)).
+    { simpl. apply ord_right. apply upper_bound_le_arrow_unknown_cov. pose (p := size_gt_0 τ1). lia. }
+  - destruct (smart_lookup A (TRec τ , TRec TUnknown)) as [[i p] | np].
+    + by apply (consp_TauGroundRecUseCall A τ i).
+    + apply consp_TauGroundRecExposeCall; auto.
+      apply (struct_validity ((TRec τ, TRec TUnknown) :: A)). constructor; simpl; auto. split; auto. done. apply (TRec_closed_unfold pτC). done.
+      assert (H : TUnknown = TUnknown.[TRec TUnknown/]). by asimpl.
+      apply GenSymUnknownR.
+      { apply ord_left. apply upper_bound_lt_rec_star; auto. }
+  - exfalso. apply (no_var_is_closed i pτC).
+Qed.
+
+
+Next Obligation. Proof. intros; simplify_eq. apply ord_right. apply upper_bound_le_prod1. simpl. pose (p := size_gt_0 τ2). lia. Qed.
+Next Obligation. Proof. intros; simplify_eq. apply ord_right. apply upper_bound_le_prod2. simpl. pose (p := size_gt_0 τ1). lia. Qed.
+Next Obligation. Proof. intros; simplify_eq. apply ord_right. apply upper_bound_le_sum1. simpl. pose (p := size_gt_0 τ2). lia. Qed.
+Next Obligation. Proof. intros; simplify_eq. apply ord_right. apply upper_bound_le_sum2. simpl. pose (p := size_gt_0 τ1). lia. Qed.
+
+
+
+(** TArrow *)
+
+Next Obligation.
+Proof.
+  intros; simplify_eq.
+  apply ord_right. apply upper_bound_le_arrow_l. simpl.
+  pose (p := size_gt_0 τ2). lia.
+Qed.
+
+
+Next Obligation.
+Proof.
+  intros; simplify_eq.
+  apply ord_right. apply upper_bound_le_arrow_r.
+  simpl. pose (p1 := size_gt_0 τ1). lia.
+Qed.
+
+(** TRec *)
+
+Next Obligation.
+Proof.
+  intros.
+  destruct (smart_lookup A (TRec τ , TRec τ')) as [[i p] | np].
+  + by apply (consp_TRecTRecUseCall A τ τ' i).
+  + apply consp_TRecTRecExposeCall; auto.
+    simplify_eq.
+    apply (struct_validity ((TRec τ, TRec τ') :: A)). constructor; simpl; auto. apply (TRec_closed_unfold pτC). apply (TRec_closed_unfold pτ'C).
+    (* apply (struct_validity ((TRec τ, TRec τ') :: A) τ.[TRec τ/] (TRec_closed_unfold pτC) τ'.[TRec τ'/] (TRec_closed_unfold pτ'C)). *)
+    by apply cons_stand_open_unfold.
+    { apply ord_left. apply upper_bound_lt_rec_rec; auto. }
+Qed.
+
+
+(** WF *)
+
+Next Obligation.
+Proof.
+  apply measure_wf.
+  apply wf_lexprod.
+  apply lt_wf. intros _.
+  apply lt_wf.
+Qed.
