theories/cast_calculus/consistency/equivalence/proof.v
@@ -1,5 +1,8 @@
 From fae_gtlc_mu Require Import prelude.
-From fae_gtlc_mu.cast_calculus.consistency Require Import standard structural.
+From fae_gtlc_mu.cast_calculus.consistency Require Import standard structural first_half second_half.
 
 Lemma cons_co τi pτi τf pτf : cons_stand τi pτi τf pτf → cons_struct [] τi τf.
-Admitted.
+Proof.
+  intro. apply cons_struct_pre_cons_struct.
+  by apply struct_validity.
+Qed.
