theories/embedding/well_typedness.v
@@ -1,0 +1,19 @@
+From fae_gtlc_mu.stlc_mu Require Export typing contexts.
+From fae_gtlc_mu.cast_calculus Require Export typing contexts.
+
+From fae_gtlc_mu.embedding Require Import types expressions.
+
+Lemma well_typedness_expr Γ e τ : (Γ ⊢ₛ e : τ) →
+    map embed_type Γ ⊢ₜ embed_expr e : embed_type τ.
+Proof.
+  induction 1; simpl; try by econstructor.
+  - constructor. by apply embd_closed. by rewrite list_lookup_fmap H.
+  - apply InjL_typed. by apply embd_closed. auto.
+  - apply InjR_typed. by apply embd_closed. auto.
+  - eapply Lam_typed. by apply embd_closed. apply IHtyped.
+  - apply Fold_typed.
+    by rewrite embd_unfold_comm in IHtyped.
+  - rewrite embd_unfold_comm.
+    by apply Unfold_typed.
+Qed.
+
