theories/refinements/static_gradual/compat_cast/all.v
@@ -8,8 +8,7 @@ From iris.program_logic Require Import lifting.
 From fae_gtlc_mu.cast_calculus Require Export types.
 From fae_gtlc_mu.cast_calculus Require Export consistency.structural.
 From fae_gtlc_mu.backtranslation Require Export cast_help.general cast_help.extract cast_help.embed.
-From fae_gtlc_mu.refinements.static_gradual.compat_cast Require Export between_rec prod_prod sum_sum arrow_arrow identity tau_star ground_star tau_star star_tau.
-(*    star_ground *)
+From fae_gtlc_mu.refinements.static_gradual.compat_cast Require Export between_rec prod_prod sum_sum arrow_arrow identity tau_star ground_star tau_star star_tau star_ground.
 
 Section compat_cast_all.
   Context `{!implG Σ,!specG Σ}.
@@ -28,8 +27,7 @@ Section compat_cast_all.
   Lemma back_cast_ar_all {A} {τi τf} (pC : cons_struct A τi τf) : back_cast_ar pC.
   Proof.
     induction pC.
-    (* - by apply back_cast_ar_star_ground. *)
-    - admit.
+    - by apply back_cast_ar_star_ground.
     - by apply back_cast_ar_ground_star.
     - by apply back_cast_ar_tau_star.
     - by apply back_cast_ar_star_tau.
@@ -40,21 +38,10 @@ Section compat_cast_all.
     - by apply back_cast_ar_arrow_arrow.
     - by apply back_cast_ar_trec_trec_expose.
     - by apply back_cast_ar_trec_trec_use.
-  Admitted.
+  Qed.
 
 
   Notation "'` H" := (bin_log_related_alt H) (at level 8).
-
-  (* Lemma interp_closed Δ τ (pτc : TClosed τ) : *)
-  (*   ⟦ τ ⟧ Δ *)
-  (*   ≡ ⟦ τ ⟧ []. *)
-  (* Proof. Admitted. *)
-
-  (* Lemma interp_closed' Δ τ vv' (pτc : TClosed τ) : *)
-  (*   ⟦ τ ⟧ Δ vv' *)
-  (*   ≡ ⟦ τ ⟧ [] vv'. *)
-  (* Proof. Admitted. *)
-
 
   Lemma bin_log_related_back_cast Γ e e' τi τf (pC : cons_struct [] τi τf)
       (IHHtyped : Γ ⊨ e ≤log≤ e' : τi) :
@@ -67,7 +54,6 @@ Section compat_cast_all.
     iApply (wp_wand with "[Hj]"). iApply ('`IHHtyped _ _ (CastCtx τi τf :: K)). iFrame. auto.
     iIntros (v). iDestruct 1 as (v') "[Hv' Hvv']". simpl.
     rewrite -𝓕c_rewrite.
-    (* rewrite (interp_closed' _ τi); auto. *)
     iApply (wp_wand with "[-]").
     iApply ((back_cast_ar_all pC) with "[-]").
     iSplitR. unfold rel_cast_functions. iSplit; auto.
