theories/refinements/static_gradual/compat_cast/star_ground.v
@@ -6,7 +6,7 @@ From iris.proofmode Require Import tactics.
 From iris.program_logic Require Import lifting.
 From fae_gtlc_mu.cast_calculus Require Export types.
 From fae_gtlc_mu.cast_calculus Require Export consistency.structural.
-From fae_gtlc_mu.backtranslation Require Export cast_help.general cast_help.extract cast_help.embed.
+From fae_gtlc_mu.backtranslation Require Export cast_help.general cast_help.extract cast_help.embed cast_help.props.extract_embed.
 From fae_gtlc_mu.cast_calculus Require Export types typing.
 
 Section star_ground.
@@ -26,152 +26,59 @@ Section star_ground.
   (*   auto. *)
   (* Qed. *)
 
+  Opaque Ω.
 
   Lemma back_cast_ar_star_ground (A : list (type * type)) (τG : type) (G : Ground τG) : back_cast_ar (consStarTGround A τG G).
   Proof.
     rewrite /back_cast_ar /𝓕c /𝓕. iIntros (ei' K' v v' fs) "(#Hfs & #Hvv' & #Hei' & Hv')". rewrite extract_no_subs.
     destruct G; rewrite interp_rw_TUnknown.
-    - (iDestruct "Hvv'" as (w w') "#[[% Hww]|[[% Hww]|[[% Hww]|[[% Hww]|[% Hww]]]]]"; inversion H; clear H H1 H2 v v').
-      + admit.
-      + admit.
-      + admit.
-      + admit.
-      + admit.
-    - (iDestruct "Hvv'" as (w w') "#[[% Hww]|[[% Hww]|[[% Hww]|[[% Hww]|[% Hww]]]]]"; inversion H; clear H H1 H2 v v').
-      + admit.
-      + admit.
-      + admit.
-      + admit.
-      + admit.
-    - (iDestruct "Hvv'" as (w w') "#[[% Hww]|[[% Hww]|[[% Hww]|[[% Hww]|[% Hww]]]]]"; inversion H; clear H H1 H2 v v').
-      + admit.
-      + admit.
-      + admit.
-      + admit.
-      + admit.
-    - (iDestruct "Hvv'" as (w w') "#[[% Hww]|[[% Hww]|[[% Hww]|[[% Hww]|[% Hww]]]]]"; inversion H; clear H H1 H2 v v').
-      + admit.
-      + admit.
-      + admit.
-      + admit.
-      + admit.
-    - (iDestruct "Hvv'" as (w w') "#[[% Hww]|[[% Hww]|[[% Hww]|[[% Hww]|[% Hww]]]]]"; inversion H; clear H H1 H2 v v').
-      + admit.
-      + admit.
-      + admit.
-      + admit.
-      + admit.
-      + admit.
-  Admitted.
+    - (iDestruct "Hvv'" as (w w') "#[[% Hww]|[[% Hww]|[[% Hww]|[[% Hww]|[% Hww]]]]]"; inversion H; clear H H1 H2 v v');
+      try by (wp_head; iApply (wp_bind (stlc_mu.lang.fill_item $ stlc_mu.lang.CaseCtx _ _)); wp_head; wp_value; repeat ((by rewrite Ω_closed; by iApply wp_Ω) || wp_head)).
+      iApply (wp_pure_step_later _ _ _ (stlc_mu.lang.of_val w) True); auto.
+      intros _. apply extract_TUnit_embed_TUnit. repeat iModIntro.
+      iMod (step_pure _ ei' K'
+                      (Cast (# castupV_TUnit w') ⋆ TUnit)
+                      w' with "[Hv']") as "Hv'".
+      eapply Same_Ground. auto. constructor. auto. auto. wp_value.
+      iExists _. auto.
+    - (iDestruct "Hvv'" as (w w') "#[[% Hww]|[[% Hww]|[[% Hww]|[[% Hww]|[% Hww]]]]]"; inversion H; clear H H1 H2 v v');
+      try by (wp_head; iApply (wp_bind (stlc_mu.lang.fill_item $ stlc_mu.lang.CaseCtx _ _)); wp_head; wp_value; repeat ((by rewrite Ω_closed; by iApply wp_Ω) || wp_head)).
+      iApply (wp_pure_step_later _ _ _ (stlc_mu.lang.of_val w) True); auto.
+      intros _. apply extract_TProd_embed_TProd. repeat iModIntro.
+      iMod (step_pure _ ei' K'
+                      (Cast (# castupV_TProd w') ⋆ (TProd ⋆ ⋆))
+                      w' with "[Hv']") as "Hv'".
+      eapply Same_Ground. auto. constructor. auto. auto. wp_value.
+      iExists _. auto.
+    - (iDestruct "Hvv'" as (w w') "#[[% Hww]|[[% Hww]|[[% Hww]|[[% Hww]|[% Hww]]]]]"; inversion H; clear H H1 H2 v v');
+      try by (wp_head; iApply (wp_bind (stlc_mu.lang.fill_item $ stlc_mu.lang.CaseCtx _ _)); wp_head; wp_value; repeat ((by rewrite Ω_closed; by iApply wp_Ω) || wp_head)).
+      iApply (wp_pure_step_later _ _ _ (stlc_mu.lang.of_val w) True); auto.
+      intros _. apply extract_TSum_embed_TSum. repeat iModIntro.
+      iMod (step_pure _ ei' K'
+                      (Cast (# castupV_TSum w') ⋆ (TSum ⋆ ⋆))
+                      w' with "[Hv']") as "Hv'".
+      eapply Same_Ground. auto. constructor. auto. auto. wp_value.
+      iExists _. auto.
+    - (iDestruct "Hvv'" as (w w') "#[[% Hww]|[[% Hww]|[[% Hww]|[[% Hww]|[% Hww]]]]]"; inversion H; clear H H1 H2 v v');
+      try by (wp_head; iApply (wp_bind (stlc_mu.lang.fill_item $ stlc_mu.lang.CaseCtx _ _)); wp_head; wp_value; repeat ((by rewrite Ω_closed; by iApply wp_Ω) || wp_head)).
+      iApply (wp_pure_step_later _ _ _ (stlc_mu.lang.of_val w) True); auto.
+      intros _. apply extract_TArrow_embed_TArrow. repeat iModIntro.
+      iMod (step_pure _ ei' K'
+                      (Cast (# castupV_TArrow w') ⋆ (TArrow ⋆ ⋆))
+                      w' with "[Hv']") as "Hv'".
+      eapply Same_Ground. auto. constructor. auto. auto. wp_value.
+      iExists _. auto.
+    - (iDestruct "Hvv'" as (w w') "#[[% Hww]|[[% Hww]|[[% Hww]|[[% Hww]|[% Hww]]]]]"; inversion H; clear H H1 H2 v v');
+      try by  (wp_head; iApply (wp_bind (stlc_mu.lang.fill_item $ stlc_mu.lang.CaseCtx _ _)); wp_head; wp_value; wp_head; by iApply wp_Ω).
 
-
-  (* Lemma back_cast_ar_star_ground (A : list (type * type)) (τG : type) (G : Ground τG) : back_cast_ar (consStarTGround A τG G). *)
-  (* Proof. *)
-  (*   rewrite /back_cast_ar /𝓕c /𝓕. iIntros (ei' K' v v' fs) "(#Hfs & #Hvv' & #Hei' & Hv')". rewrite extract_no_subs. *)
-  (*   destruct G. *)
-  (*   - (** TUnit *) rewrite unfold_fixpoint_interp_unknown1'; try by constructor. *)
-  (*     iDestruct "Hvv'" as "[Hvv'Unit|[Hpp'|[Hss'|[Hff'|Huu']]]]". *)
-  (*     * iDestruct "Hvv'Unit" as "%"; inversion H; clear v v' H H1 H2. *)
-  (*       (** easy case; delegate to extract_embed file with good tactics *) *)
-  (*       admit. *)
-
-  (*       (* iApply wp_pure_step_later; auto; iNext; asimpl. *) *)
-  (*       (* iApply (wp_bind (stlc_mu.lang.fill_item $ stlc_mu.lang.CaseCtx _ _)). *) *)
-  (*       (* iApply wp_pure_step_later; auto; iNext. *) *)
-  (*       (* iApply wp_value. *) *)
-  (*       (* iApply wp_pure_step_later; auto; iNext. *) *)
-  (*       (* iApply wp_pure_step_later; auto; iNext. asimpl. *) *)
-  (*       (* iApply wp_pure_step_later; auto; iNext. *) *)
-  (*       (* iApply wp_pure_step_later; auto; iNext. asimpl. *) *)
-  (*       (* iMod (step_pure _ ei' K' (Cast (Cast Unit TUnit ⋆) ⋆ TUnit) (# UnitV) with "[Hv']") as "HHHH"; intros; auto. *) *)
-  (*       (* apply Same_Ground with (v := UnitV ); auto; constructor. *) *)
-  (*       (* iApply wp_value. *) *)
-  (*       (* iExists UnitV. *) *)
-  (*       (* by repeat iFrame. *) *)
-
-
-  (*     * iDestruct "Hpp'" as (v1 v1' v2 v2') "(% & #H1 & #H2)". simpl in H; inversion H; clear H H1 H2 v v'. *)
-  (*       repeat rewrite (refold_interp_unknown'). *)
-  (*       (** diverging case *) *)
-  (*       admit. *)
-
-  (*         (* asimpl. *) *)
-  (*         (* iApply wp_pure_step_later; auto; iNext; asimpl. *) *)
-  (*         (* iApply (wp_bind (stlc_mu.lang.fill_item $ stlc_mu.lang.CaseCtx _ _)). *) *)
-  (*         (* iApply wp_pure_step_later; auto; iNext. *) *)
-  (*         (* iApply wp_value. *) *)
-  (*         (* iApply wp_pure_step_later; auto; iNext; asimpl. *) *)
-  (*         (* iApply wp_pure_step_later; auto; iNext; asimpl. *) *)
-  (*         (* iApply wp_pure_step_later; auto; iNext. asimpl. *) *)
-  (*         (* by iApply wp_Ω. *) *)
-
-
-
-  (*     * iDestruct "Hss'" as "[H1 | H2]". *)
-  (*       -- iDestruct "H1" as (v1 v1') "[% Hv1v1']"; rewrite (refold_interp_unknown'); inversion H; clear H H1 H2 v v'. *)
-  (*          (** diverging case *) admit. *)
-  (*         -- iDestruct "H2" as (v2 v2') "[% Hv2v2']"; rewrite (refold_interp_unknown'); inversion H; clear H H1 H2 v v'. *)
-  (*          (** diverging case *) admit. *)
-  (*     * iDestruct "Hff'" as (f f') "[% Hff']". inversion H. clear H H1 H2 v v'. *)
-  (*       (** diverging case *) admit. *)
-  (*     * iDestruct "Huu'" as (u u') "[% H]"; rewrite (refold_interp_unknown'); inversion H; clear H H1 H2 v v'. *)
-  (*       (** diverging case *) admit. *)
-  (*   - (** TProd *) *)
-  (*     admit. *)
-  (*   - (** TSum *) admit. *)
-  (*   - (** TArrow *) rewrite unfold_fixpoint_interp_unknown1'. *)
-  (*     iDestruct "Hvv'" as "[Hvv'Unit|[Hpp'|[Hss'|[Hff'|Huu']]] ]". *)
-  (*     * iDestruct "Hvv'Unit" as "%"; inversion H; clear v v' H H1 H2. *)
-  (*       (** diverging case *) admit. *)
-  (*     * iDestruct "Hpp'" as (v1 v1' v2 v2') "(% & #H1 & #H2)". simpl in H; inversion H; clear H H1 H2 v v'. *)
-  (*       repeat rewrite (refold_interp_unknown'). *)
-  (*       (** diverging case *) admit. *)
-  (*     * iDestruct "Hss'" as "[H1 | H2]". *)
-  (*       -- iDestruct "H1" as (v1 v1') "[% Hv1v1']"; rewrite (refold_interp_unknown'); inversion H; clear H H1 H2 v v'. *)
-  (*           (** diverging case *) admit. *)
-  (*       -- iDestruct "H2" as (v2 v2') "[% Hv2v2']"; rewrite (refold_interp_unknown'); inversion H; clear H H1 H2 v v'. *)
-  (*           (** diverging case *) admit. *)
-  (*     * iDestruct "Hff'" as (f f') "[% Hff']". inversion H. clear H H1 H2 v v'. *)
-  (*       (** easy case *) admit. *)
-  (*     * iDestruct "Huu'" as (u u') "[% H]"; rewrite (refold_interp_unknown'); inversion H; clear H H1 H2 v v'. *)
-  (*       (** diverging case *) admit. *)
-  (*     * constructor. *)
-  (*   - (** TRec *) rewrite unfold_fixpoint_interp_unknown1'. *)
-  (*     iDestruct "Hvv'" as "[Hvv'Unit|[Hpp'|[Hss'|[Hff'|Huu']]] ]". *)
-  (*     * iDestruct "Hvv'Unit" as "%"; inversion H; clear v v' H H1 H2. *)
-  (*       (** diverging case *) admit. *)
-  (*     * iDestruct "Hpp'" as (v1 v1' v2 v2') "(% & #H1 & #H2)". simpl in H; inversion H; clear H H1 H2 v v'. *)
-  (*       repeat rewrite (refold_interp_unknown'). *)
-  (*       (** diverging case *) admit. *)
-  (*     * iDestruct "Hss'" as "[H1 | H2]". *)
-  (*       -- iDestruct "H1" as (v1 v1') "[% Hv1v1']"; rewrite (refold_interp_unknown'); inversion H; clear H H1 H2 v v'. *)
-  (*          (** diverging case *) admit. *)
-  (*       -- iDestruct "H2" as (v2 v2') "[% Hv2v2']"; rewrite (refold_interp_unknown'); inversion H; clear H H1 H2 v v'. *)
-  (*          (** diverging case *) admit. *)
-  (*     * iDestruct "Hff'" as (f f') "[% Hff']". inversion H. clear H H1 H2 v v'. *)
-  (*       (** diverging case *) admit. *)
-  (*     * iDestruct "Huu'" as (u u') "[% #H]"; rewrite (refold_interp_unknown'); inversion H; clear H H1 H2 v v'. *)
-  (*       (** easy case*) *)
-  (*       rewrite /embedV_TUnknown /castupV_TRec. *)
-  (*       iMod (step_pure _ ei' K' *)
-  (*                         (Cast (# castupV_TRec (FoldV u')) ⋆ (TRec ⋆)) *)
-  (*                         (# (FoldV u')) *)
-  (*                 with "[Hv']") as "HHHH"; auto. *)
-  (*       eapply Same_Ground. apply to_of_val. constructor. *)
-  (*       iApply wp_pure_step_later; auto; iNext; asimpl. *)
-  (*       iApply (wp_bind (stlc_mu.lang.fill_item $ stlc_mu.lang.CaseCtx _ _)). *)
-  (*       iApply wp_pure_step_later; auto. *)
-  (*       iApply wp_value. simpl. *)
-  (*       iApply wp_pure_step_later; auto. asimpl. *)
-  (*       iApply wp_value. *)
-  (*       repeat iNext. *)
-  (*       iExists (FoldV u'). iSplitL. done. *)
-  (*       rewrite fixpoint_interp_rec1_eq. *)
-  (*       iModIntro. *)
-  (*       iExists (u, u'). *)
-  (*       iSplitL; done. *)
-  (*     * constructor. *)
-  (* Admitted. *)
-
+      iApply (wp_pure_step_later _ _ _ (stlc_mu.lang.Fold (stlc_mu.lang.of_val w)) True); auto.
+      intros _. apply extract_TRec_embed_TUnknown. repeat iModIntro.
+      iMod (step_pure _ ei' K'
+                      (Cast (# castupV_TRec (FoldV w')) ⋆ (TRec ⋆))
+                      (FoldV w') with "[Hv']") as "Hv'".
+      eapply Same_Ground. auto. constructor. auto. auto. wp_value.
+      iExists _. rewrite interp_rw_TRec. asimpl. iSplit; auto. by simpl.
+      Unshelve. all:apply hacki.
+  Qed.
 
 End star_ground.
