theories/refinements/static_gradual/rel_ref_specs.v
@@ -1,162 +1,98 @@
 From fae_gtlc_mu.refinements.static_gradual Require Export logical_relation compat_easy.
-(* From fae_gtlc_mu.embedding Require Import expressions types. *)
+From fae_gtlc_mu.embedding Require Import expressions types.
 From fae_gtlc_mu.stlc_mu Require Export typing.
 From fae_gtlc_mu.cast_calculus Require Export types.
-
-
-(* Ltac fold_interp := *)
-(*   match goal with *)
-(*   | |- context [ interp_expr (interp_arrow (interp ?A) (interp ?A')) *)
-(*                             ?B (?C, ?D) ] => *)
-(*     change (interp_expr (interp_arrow (interp A) (interp A')) B (C, D)) with *)
-(*     (interp_expr (interp (TArrow A A')) B (C, D)) *)
-(*   | |- context [ interp_expr (interp_prod (interp ?A) (interp ?A')) *)
-(*                             ?B (?C, ?D) ] => *)
-(*     change (interp_expr (interp_prod (interp A) (interp A')) B (C, D)) with *)
-(*     (interp_expr (interp (TProd A A')) B (C, D)) *)
-(*   | |- context [ interp_expr (interp_prod (interp ?A) (interp ?A')) *)
-(*                             ?B (?C, ?D) ] => *)
-(*     change (interp_expr (interp_prod (interp A) (interp A')) B (C, D)) with *)
-(*     (interp_expr (interp (TProd A A')) B (C, D)) *)
-(*   | |- context [ interp_expr (interp_sum (interp ?A) (interp ?A')) *)
-(*                             ?B (?C, ?D) ] => *)
-(*     change (interp_expr (interp_sum (interp A) (interp A')) B (C, D)) with *)
-(*     (interp_expr (interp (TSum A A')) B (C, D)) *)
-(*   | |- context [ interp_expr (interp_rec (interp ?A)) ?B (?C, ?D) ] => *)
-(*     change (interp_expr (interp_rec (interp A)) B (C, D)) with *)
-(*     (interp_expr (interp (TRec A)) B (C, D)) *)
-(*   end. *)
 
 Section relation_for_specification_lemma.
   Context `{!implG Σ, !specG Σ}.
 
-  (* Notation "Γ ⊨ e '≤log≤' e' : τ" := *)
-    (* (bin_log_related Γ e e' τ) (at level 74, e, e', τ at next level). *)
-
-  (* Theorem embedding_relates (Γ : list stlc_mu.typing.type) pΓ (e : stlc_mu.lang.expr) (τ : stlc_mu.typing.type) pτ : *)
-  (*   Γ ⊢ₛ e : τ → map embed_type Γ ⊨ e ≤log≤ [[e]] : [| τ |]. *)
-  (* Proof. *)
-  (*   induction 1; simpl. *)
-  (*   - apply bin_log_related_var. by rewrite list_lookup_fmap H. *)
-  (*   - by apply bin_log_related_unit. *)
-  (*   - apply bin_log_related_pair; eauto. *)
-  (*   - eapply bin_log_related_fst; eauto. *)
-  (*   - eapply bin_log_related_snd; eauto. *)
-  (*   - eapply bin_log_related_injl; eauto. *)
-  (*   - eapply bin_log_related_injr; eauto. *)
-  (*   - eapply bin_log_related_case; try done; *)
-  (*       ((by (rewrite map_length; match goal with H : _ |- _ => eapply (stlc_mu.typing.typed_n_closed _ _ _ H) end)) || *)
-  (*        (try done)). *)
-  (*     admit. *)
-  (*     admit. *)
-  (*   - eapply bin_log_related_lam; eauto. *)
-  (*     rewrite map_length. *)
-  (*       match goal with H : _ |- _ => eapply (stlc_mu.typing.typed_n_closed _ _ _ H) end. *)
-  (*       admit. *)
-  (*   - eapply bin_log_related_app; eauto. *)
-  (*   - eapply bin_log_related_fold; eauto. *)
-  (*     by rewrite -embed_through_unfold. *)
-  (*   - rewrite embed_through_unfold. eapply bin_log_related_unfold; eauto. *)
-  (* Admitted. *)
+  Theorem embedding_relates (Γ : list stlc_mu.types.type) (e : stlc_mu.lang.expr) (τ : stlc_mu.types.type) :
+    Γ ⊢ₛ e : τ → map embed_type Γ ⊨ e ≤log≤ [[e]] : [| τ |].
+  Proof.
+    induction 1; simpl.
+    - apply bin_log_related_var. by rewrite list_lookup_fmap H.
+    - by apply bin_log_related_unit.
+    - by apply bin_log_related_pair.
+    - by eapply bin_log_related_fst.
+    - by eapply bin_log_related_snd.
+    - by apply bin_log_related_injl.
+    - by apply bin_log_related_injr.
+    - by eapply bin_log_related_case.
+    - by apply bin_log_related_lam.
+    - by eapply bin_log_related_app.
+    - apply bin_log_related_fold. by rewrite -embd_unfold_comm.
+    - rewrite embd_unfold_comm. apply bin_log_related_unfold. by simpl in IHtyped.
+  Qed.
 
   From fae_gtlc_mu.refinements.static_gradual Require Import compat_cast.all.
   From fae_gtlc_mu.backtranslation Require Import expressions well_typedness.
 
-  Theorem back_relates (Γ : list cast_calculus.types.type) pΓ (e : cast_calculus.lang.expr) (τ : cast_calculus.types.type) pτ :
-    Γ & pΓ ⊢ₜ e : τ & pτ → Γ ⊨ <<e>> ≤log≤ e : τ.
+  Theorem back_relates (Γ : list cast_calculus.types.type) (e : cast_calculus.lang.expr) (τ : cast_calculus.types.type) :
+    Γ ⊢ₜ e : τ → Γ ⊨ <<e>> ≤log≤ e : τ.
   Proof.
     induction 1; simpl.
     - by apply bin_log_related_var.
     - by apply bin_log_related_unit.
-    - apply bin_log_related_pair; eauto.
-    - eapply bin_log_related_fst; eauto.
-    - eapply bin_log_related_snd; eauto.
-    - eapply bin_log_related_injl; eauto.
-    - eapply bin_log_related_injr; eauto.
-    - eapply bin_log_related_case; try done.
-      cut (∀ f : var → stlc_mu.lang.expr, (<< e1 >>).[upn (length (map backtranslate_type (τ1 :: Γ))) f] = << e1 >>).
-      { rewrite map_length. by simpl. }
-      eapply stlc_mu.typing.typed_n_closed. apply well_typedness_expr. apply H0.
-      cut (∀ f : var → stlc_mu.lang.expr, (<< e2 >>).[upn (length (map backtranslate_type (τ2 :: Γ))) f] = << e2 >>).
-      { rewrite map_length. by simpl. }
-      eapply stlc_mu.typing.typed_n_closed. apply well_typedness_expr. apply H1.
-      rewrite -(cons_length τ1). by eapply cast_calculus.typing.typed_n_closed.
-      rewrite -(cons_length τ2). by eapply cast_calculus.typing.typed_n_closed.
-    - eapply bin_log_related_lam; eauto.
-      cut (∀ f : var → stlc_mu.lang.expr, (<< e >>).[upn (length (map backtranslate_type (τ1 :: Γ))) f] = << e >>).
-      { rewrite map_length. by simpl. }
-      eapply stlc_mu.typing.typed_n_closed. apply well_typedness_expr. apply H.
-      rewrite -(cons_length τ1). by eapply cast_calculus.typing.typed_n_closed.
-    - eapply bin_log_related_app; eauto.
-    - eapply bin_log_related_fold; eauto.
-    - eapply bin_log_related_unfold; eauto.
-    - destruct (decide (cons_stand_open τi τf));
+    - by apply bin_log_related_pair.
+    - by eapply bin_log_related_fst.
+    - by eapply bin_log_related_snd.
+    - by apply bin_log_related_injl.
+    - by apply bin_log_related_injr.
+    - by eapply bin_log_related_case.
+    - by apply bin_log_related_lam.
+    - by eapply bin_log_related_app.
+    - by apply bin_log_related_fold.
+    - by apply bin_log_related_unfold.
+    - assert (pτi : cast_calculus.types.TClosed τi). apply (cast_calculus.typing.typed_closed H).
+      destruct (cons_stand_open_dec τi τf);
                 destruct (decide (cast_calculus.types.TClosed τi));
                 destruct (decide (cast_calculus.types.TClosed τf)); try by contradiction.
       by apply bin_log_related_back_cast.
     - apply bin_log_related_omega.
   Qed.
 
-  (* From fae_gtlc_mu.stlc_mu Require Export contexts. *)
-  (* From fae_gtlc_mu.cast_calculus Require Export contexts. *)
-  (* From fae_gtlc_mu.backtranslation Require Import contexts. *)
+  From fae_gtlc_mu.stlc_mu Require Export contexts.
+  From fae_gtlc_mu.cast_calculus Require Export contexts.
+  From fae_gtlc_mu.backtranslation Require Import contexts.
 
-  (* Lemma back_ctx_relates (Γ : list stlc_mu.typing.type) (e : stlc_mu.lang.expr) (e' : cast_calculus.lang.expr) *)
-  (*       (τ : stlc_mu.typing.type) (Γ' : list cast_calculus.types.type) (τ' : cast_calculus.types.type) (C : cast_calculus.contexts.ctx) : *)
-  (*   (∀ f, e.[upn (length Γ) f] = e) → *)
-  (*   (∀ f, e'.[upn (length Γ) f] = e') → *)
-  (*     cast_calculus.contexts.typed_ctx C (map embed_type Γ) [|τ|] Γ' τ' → *)
-  (*     map embed_type Γ ⊨ e ≤log≤ e' : [| τ |] → *)
-  (*     Γ' ⊨ stlc_mu.contexts.fill_ctx (backtranslate_ctx C) e ≤log≤ cast_calculus.contexts.fill_ctx C e' : τ'. *)
-  (* Proof. *)
-  (*   revert Γ τ Γ' τ' e e'. *)
-  (*   induction C as [aa |c C] => Γ τ Γ' τ' e e' H1 H2; simpl. *)
-  (*   - by intros; inversion_clear H. *)
-  (*   - inversion_clear 1 as [aa |? ? ? ? ? ? ? ? Hx1 Hx2]. intros H3. *)
-  (*     specialize (IHC _ _ _ _ e e' H1 H2 Hx2 H3). *)
-  (*     inversion Hx1; subst; simpl; try fold_interp. *)
-  (*     + eapply bin_log_related_lam. *)
-  (*       admit. *)
-  (*       admit. *)
-  (*       admit. *)
-  (*       (* eauto; *) *)
-  (*         (* match goal with *) *)
-  (*           (* H : _ |- _ => eapply (typed_ctx_n_closed _ _ _ _ _ _ _ H) *) *)
-  (*         (* end. *) *)
-  (*     + eapply bin_log_related_app; eauto using back_relates. *)
-  (*     + eapply bin_log_related_app; eauto using back_relates. *)
-  (*     + eapply bin_log_related_pair; eauto using back_relates. *)
-  (*     + eapply bin_log_related_pair; eauto using back_relates. *)
-  (*     + eapply bin_log_related_fst; eauto. *)
-  (*     + eapply bin_log_related_snd; eauto. *)
-  (*     + eapply bin_log_related_injl; eauto. *)
-  (*     + eapply bin_log_related_injr; eauto. *)
-  (*     + eapply bin_log_related_case; try done; try apply back_relates. *)
-  (*       admit. *)
-  (*       admit. *)
-  (*       admit. *)
-  (*       admit. *)
-  (*       admit. *)
-  (*       admit. *)
-  (*     + eapply bin_log_related_case; try done; try apply back_relates. *)
-  (*       admit. *)
-  (*       admit. *)
-  (*       admit. *)
-  (*       admit. *)
-  (*       admit. *)
-  (*       admit. *)
-  (*     + eapply bin_log_related_case; try done; try apply back_relates. *)
-  (*       admit. *)
-  (*       admit. *)
-  (*       admit. *)
-  (*       admit. *)
-  (*       admit. *)
-  (*       admit. *)
-  (*     + eapply bin_log_related_fold; eauto. *)
-  (*     + eapply bin_log_related_unfold; eauto. *)
-  (*     + destruct (cons_stand_dec τ2 τ'); destruct (decide (TClosed τ2)); destruct (decide (TClosed τ')); try by contradiction. *)
-  (*       simpl. *)
-  (*       by apply bin_log_related_back_cast. *)
-  (* Admitted. *)
+  Lemma back_ctx_item_relates (Γ : list cast_calculus.types.type) (e : stlc_mu.lang.expr) (e' : cast_calculus.lang.expr) (τ : cast_calculus.types.type) (pτ : TClosed τ)
+        (Γ' : list cast_calculus.types.type) (τ' : cast_calculus.types.type) (C : cast_calculus.contexts.ctx_item) :
+      cast_calculus.contexts.typed_ctx_item C Γ τ Γ' τ' →
+      Γ ⊨ e ≤log≤ e' : τ →
+      Γ' ⊨ stlc_mu.contexts.fill_ctx_item (backtranslate_ctx_item C) e ≤log≤ cast_calculus.contexts.fill_ctx_item C e' : τ'.
+  Proof.
+    destruct C; intros; inversion H; simplify_eq; simpl.
+    - by apply bin_log_related_lam.
+    - eapply bin_log_related_app; eauto using back_relates.
+    - eapply bin_log_related_app; eauto using back_relates.
+    - eapply bin_log_related_pair; eauto using back_relates.
+    - eapply bin_log_related_pair; eauto using back_relates.
+    - by eapply bin_log_related_fst.
+    - by eapply bin_log_related_snd.
+    - by apply bin_log_related_injl.
+    - by apply bin_log_related_injr.
+    - eapply bin_log_related_case; try apply back_relates; try done.
+    - eapply bin_log_related_case; try apply back_relates; try done.
+    - eapply bin_log_related_case; try apply back_relates; try done.
+    - by apply bin_log_related_fold.
+    - by apply bin_log_related_unfold.
+    - destruct (cons_stand_open_dec τ τ');
+                destruct (decide (cast_calculus.types.TClosed τ));
+                destruct (decide (cast_calculus.types.TClosed τ')); try by contradiction.
+      by apply bin_log_related_back_cast.
+  Qed.
+
+  Lemma back_ctx_relates (Γ : list cast_calculus.types.type) (e : stlc_mu.lang.expr) (e' : cast_calculus.lang.expr) (τ : cast_calculus.types.type) (pτ : TClosed τ)
+        (Γ' : list cast_calculus.types.type) (τ' : cast_calculus.types.type) (C : cast_calculus.contexts.ctx) :
+      cast_calculus.contexts.typed_ctx C Γ τ Γ' τ' →
+      Γ ⊨ e ≤log≤ e' : τ →
+      Γ' ⊨ stlc_mu.contexts.fill_ctx (backtranslate_ctx C) e ≤log≤ cast_calculus.contexts.fill_ctx C e' : τ'.
+  Proof.
+    revert Γ τ pτ Γ' τ' e e'.
+    induction C; intros Γ τ pτ Γ' τ' e e' H.
+    - by inversion H.
+    - inversion_clear H. intro Hee'. simpl.
+      apply back_ctx_item_relates with (Γ := Γ2) (τ := τ2). by eapply typed_ctx_closedness. auto. by eapply IHC.
+  Qed.
 
 End relation_for_specification_lemma.
